Use Add,Mul and Neg notations

ovn/src/ovn_group.rs
@@ -12,12 +12,12 @@ pub use crate::ovn_traits::*;
 // Useful definitions //
 ////////////////////////
 
-fn sub<Z : Field>(x: Z, y: Z) -> Z {
-    Z::add(x, Z::opp(y))
+fn sub<Z: Field>(x: Z, y: Z) -> Z {
+    x + /* field addition */ (-/* field opposite */y)
 }
 
-fn div<G : Group>(x: G, y: G) -> G {
-    G::prod(x, G::group_inv(y))
+fn div<G: Group>(x: G, y: G) -> G {
+    x * G::group_inv(y) // group product
 }
 
 ////////////////////
@@ -34,15 +34,11 @@ pub struct SchnorrZKPCommit<G: Group> {
 /** Non-interactive Schnorr proof using Fiat-Shamir heuristics (RFC 8235) */
 // https://www.rfc-editor.org/rfc/rfc8235
 // https://crypto.stanford.edu/cs355/19sp/lec5.pdf
-pub fn schnorr_zkp<G: Group>(
-    random: G::Z,
-    h: G,
-    x: G::Z,
-) -> SchnorrZKPCommit<G> {
+pub fn schnorr_zkp<G: Group>(random: G::Z, h: G, x: G::Z) -> SchnorrZKPCommit<G> {
     let r = random;
     let u = G::g_pow(r);
     let c = G::hash(vec![G::g(), h, u]);
-    let z = G::Z::add(r, G::Z::mul(c, x));
+    let z = r + /* field addition */ c * /* field product */ x;
 
     return SchnorrZKPCommit {
         schnorr_zkp_u: u,
@@ -52,12 +48,10 @@ pub fn schnorr_zkp<G: Group>(
 }
 
 // https://crypto.stanford.edu/cs355/19sp/lec5.pdf
-pub fn schnorr_zkp_validate<G: Group>(
-    h: G,
-    pi: SchnorrZKPCommit<G>,
-) -> bool {
+pub fn schnorr_zkp_validate<G: Group>(h: G, pi: SchnorrZKPCommit<G>) -> bool {
     pi.schnorr_zkp_c == G::hash(vec![G::g(), h, pi.schnorr_zkp_u])
-        && G::g_pow(pi.schnorr_zkp_z) == G::prod(pi.schnorr_zkp_u, G::pow(h, pi.schnorr_zkp_c))
+        && G::g_pow(pi.schnorr_zkp_z)
+            == pi.schnorr_zkp_u * /* group product */ G::pow(h, pi.schnorr_zkp_c)
 }
 
 #[derive(Serialize, SchemaType, Clone, Copy)]
@@ -94,10 +88,10 @@ pub fn zkp_one_out_of_two<G: Group>(
         let d1 = random_d;
 
         let x = G::g_pow(xi);
-        let y = G::prod(G::pow(h, xi), G::g());
+        let y = G::pow(h, xi) * /* group product */ G::g();
 
-        let a1 = G::prod(G::g_pow(r1), G::pow(x, d1));
-        let b1 = G::prod(G::pow(h, r1), G::pow(y, d1));
+        let a1 = G::g_pow(r1) * /* group product */ G::pow(x, d1);
+        let b1 = G::pow(h, r1) * /* group product */ G::pow(y, d1);
 
         let a2 = G::g_pow(w);
         let b2 = G::pow(h, w);
@@ -105,7 +99,7 @@ pub fn zkp_one_out_of_two<G: Group>(
         let c = G::hash(vec![x, y, a1, b1, a2, b2]);
 
         let d2 = sub::<G::Z>(c, d1);
-        let r2 = sub::<G::Z>(w, G::Z::mul(xi, d2));
+        let r2 = sub::<G::Z>(w, xi * /* field product */ d2);
 
         OrZKPCommit {
             or_zkp_x: x,
@@ -130,13 +124,13 @@ pub fn zkp_one_out_of_two<G: Group>(
         let a1 = G::g_pow(w);
         let b1 = G::pow(h, w);
 
-        let a2 = G::prod(G::g_pow(r2), G::pow(x, d2));
-        let b2 = G::prod(G::pow(h, r2), G::pow(div::<G>(y, G::g()), d2));
+        let a2 = G::g_pow(r2) * /* group product */ G::pow(x, d2);
+        let b2 = G::pow(h, r2) * /* group product */ G::pow(div::<G>(y, G::g()), d2);
 
         let c = G::hash(vec![x, y, a1, b1, a2, b2]);
 
         let d1 = sub::<G::Z>(c, d2);
-        let r1 = sub::<G::Z>(w, G::Z::mul(xi, d1));
+        let r1 = sub::<G::Z>(w, xi * /* field product */ d1);
 
         OrZKPCommit {
             or_zkp_x: x,
@@ -155,10 +149,7 @@ pub fn zkp_one_out_of_two<G: Group>(
 }
 
 // Anonymous voting by two-round public discussion
-pub fn zkp_one_out_of_two_validate<G: Group>(
-    h: G,
-    zkp: OrZKPCommit<G>,
-) -> bool {
+pub fn zkp_one_out_of_two_validate<G: Group>(h: G, zkp: OrZKPCommit<G>) -> bool {
     let c = G::hash(vec![
         zkp.or_zkp_x,
         zkp.or_zkp_y,
@@ -168,29 +159,23 @@ pub fn zkp_one_out_of_two_validate<G: Group>(
         zkp.or_zkp_b2,
     ]); // TODO: add i
 
-    (c == G::Z::add(zkp.or_zkp_d1, zkp.or_zkp_d2)
-        && zkp.or_zkp_a1 == G::prod(G::g_pow(zkp.or_zkp_r1), G::pow(zkp.or_zkp_x, zkp.or_zkp_d1))
+    (c == zkp.or_zkp_d1 + /* field addition */ zkp.or_zkp_d2
+        && zkp.or_zkp_a1
+            == G::g_pow(zkp.or_zkp_r1) * /* group product */ G::pow(zkp.or_zkp_x, zkp.or_zkp_d1)
         && zkp.or_zkp_b1
-            == G::prod(
-                G::pow(h, zkp.or_zkp_r1),
-                G::pow(zkp.or_zkp_y, zkp.or_zkp_d1),
-            )
-        && zkp.or_zkp_a2 == G::prod(G::g_pow(zkp.or_zkp_r2), G::pow(zkp.or_zkp_x, zkp.or_zkp_d2))
+            == G::pow(h, zkp.or_zkp_r1) * /* group product */
+                G::pow(zkp.or_zkp_y, zkp.or_zkp_d1)
+        && zkp.or_zkp_a2
+            == G::g_pow(zkp.or_zkp_r2) * /* group product */ G::pow(zkp.or_zkp_x, zkp.or_zkp_d2)
         && zkp.or_zkp_b2
-            == G::prod(
-                G::pow(h, zkp.or_zkp_r2),
-                G::pow(div::<G>(zkp.or_zkp_y, G::g()), zkp.or_zkp_d2),
-            ))
+            == G::pow(h, zkp.or_zkp_r2) * /* group product */ G::pow(div::<G>(zkp.or_zkp_y, G::g()), zkp.or_zkp_d2))
 }
 
 pub fn commit_to<G: Group>(g_pow_xi_yi_vi: G) -> G::Z {
     G::hash(vec![g_pow_xi_yi_vi])
 }
 
-pub fn check_commitment<G: Group>(
-    g_pow_xi_yi_vi: G,
-    commitment: G::Z,
-) -> bool {
+pub fn check_commitment<G: Group>(g_pow_xi_yi_vi: G, commitment: G::Z) -> bool {
     G::hash(vec![g_pow_xi_yi_vi]) == commitment
 }
 
@@ -208,7 +193,7 @@ pub struct OvnContractState<G: Group, const n: usize> {
 
     pub tally: u32,
 
-    pub round1 : [bool; n],
+    pub round1: [bool; n],
 }
 
 #[hax::init(contract = "OVN")]
@@ -246,7 +231,7 @@ pub fn init_ovn_contract<G: Group, const n: usize>(// _: &impl HasInitContext,
         tally: 0,
 
         round1: [false; n],
-   })
+    })
 }
 
 #[derive(Serialize, SchemaType)]
@@ -286,38 +271,29 @@ pub struct CastVoteParam<Z: Field> {
     pub cvp_vote: bool,
 }
 
-pub fn compute_g_pow_yi<G: Group, const n: usize>(
-    i: usize,
-    xis: [G; n],
-) -> G {
-    let mut prod1 = G::group_one();
-    for j in 0..i {
-        prod1 = G::prod(prod1, xis[j]);
-    }
+// impl<G : Group> core::ops::Mul for G {
+//     type Output = Self;
+//     fn mul (self, rhs: Self) {
+//         Self::prod(self, rhs)
+//     }
+// }
 
-    let mut prod2 = G::group_one();
-    for j in (i + 1)..n {
-        prod2 = G::prod(prod2, xis[j]);
-    }
+pub fn compute_g_pow_yi<G: Group, const n: usize>(i: usize, xis: [G; n]) -> G {
+    let mut prod1 = xis[0..i].iter().map(|x| x.clone()).product::<G>();
+    let mut prod2 = xis[i + 1..n].iter().map(|x| x.clone()).product::<G>();
 
     // implicitly: Y_i = g^y_i
     let g_pow_yi = div::<G>(prod1, prod2);
     g_pow_yi
 }
 
-pub fn compute_group_element_for_vote<G: Group>(
-    xi: G::Z,
-    vote: bool,
-    g_pow_yi: G,
-) -> G {
-    G::prod(
-        G::pow(g_pow_yi, xi),
+pub fn compute_group_element_for_vote<G: Group>(xi: G::Z, vote: bool, g_pow_yi: G) -> G {
+    G::pow(g_pow_yi, xi) * /* group product */
         G::g_pow(if vote {
             G::Z::field_one()
         } else {
             G::Z::field_zero()
-        }),
-    )
+        })
 }
 
 /** Commitment before round 2 */
@@ -395,9 +371,10 @@ pub fn tally_votes<G: Group, const n: usize, A: HasActions>(
 
     let mut vote_result = G::group_one();
     for g_pow_vote in state.g_pow_xi_yi_vis {
-        vote_result = G::prod(vote_result, g_pow_vote);
+        vote_result = vote_result * /* group product */ g_pow_vote;
     }
 
+    // let tally = (0..(n as u32)).rposition(|i| G::g_pow(i) == vote_result).unwrap() as u32;
     let mut tally = 0;
     let mut curr = G::Z::field_zero();
     for i in 0..n as u32 {
@@ -406,7 +383,7 @@ pub fn tally_votes<G: Group, const n: usize, A: HasActions>(
             tally = i;
         }
 
-        curr = G::Z::add(curr, G::Z::field_one());
+        curr = curr + /* field addition */ G::Z::field_one();
     }
 
     let mut tally_votes_state_ret = state.clone();
