ovn/proofs/fstar/extraction/Hacspec_ovn.Ovn_group.fst
@@ -1,0 +1,949 @@
+module Hacspec_ovn.Ovn_group
+#set-options "--fuel 0 --ifuel 1 --z3rlimit 15"
+open Core
+open FStar.Mul
+
+let _ =
+  (* This module has implicit dependencies, here we make them explicit. *)
+  (* The implicit dependencies arise from typeclasses instances. *)
+  let open Concordium_contracts_common.Traits in
+  let open Hacspec_concordium.Concordium_traits in
+  let open Hacspec_ovn.Ovn_traits in
+  ()
+
+type t_TallyParameter = | TallyParameter : t_TallyParameter
+
+let sub
+      (#v_Z: Type0)
+      (#[FStar.Tactics.Typeclasses.tcresolve ()] i1: Hacspec_ovn.Ovn_traits.t_Field v_Z)
+      (x y: v_Z)
+    : v_Z =
+  Hacspec_ovn.Ovn_traits.f_add #v_Z
+    #FStar.Tactics.Typeclasses.solve
+    x
+    (Hacspec_ovn.Ovn_traits.f_opp #v_Z #FStar.Tactics.Typeclasses.solve y <: v_Z)
+
+let check_commitment
+      (#v_G: Type0)
+      (#[FStar.Tactics.Typeclasses.tcresolve ()] i1: Hacspec_ovn.Ovn_traits.t_Group v_G)
+      (g_pow_xi_yi_vi: v_G)
+      (commitment: i1.f_Z)
+    : bool =
+  (Hacspec_ovn.Ovn_traits.f_hash #v_G
+      #FStar.Tactics.Typeclasses.solve
+      (Alloc.Slice.impl__into_vec #v_G
+          #Alloc.Alloc.t_Global
+          (Rust_primitives.unsize (Rust_primitives.Hax.box_new (let list = [g_pow_xi_yi_vi] in
+                    FStar.Pervasives.assert_norm (Prims.eq2 (List.Tot.length list) 1);
+                    Rust_primitives.Hax.array_of_list 1 list)
+                <:
+                Alloc.Boxed.t_Box (t_Array v_G (sz 1)) Alloc.Alloc.t_Global)
+            <:
+            Alloc.Boxed.t_Box (t_Slice v_G) Alloc.Alloc.t_Global)
+        <:
+        Alloc.Vec.t_Vec v_G Alloc.Alloc.t_Global)
+    <:
+    i1.f_Z) =.
+  commitment
+
+let commit_to
+      (#v_G: Type0)
+      (#[FStar.Tactics.Typeclasses.tcresolve ()] i1: Hacspec_ovn.Ovn_traits.t_Group v_G)
+      (g_pow_xi_yi_vi: v_G)
+    : i1.f_Z =
+  Hacspec_ovn.Ovn_traits.f_hash #v_G
+    #FStar.Tactics.Typeclasses.solve
+    (Alloc.Slice.impl__into_vec #v_G
+        #Alloc.Alloc.t_Global
+        (Rust_primitives.unsize (Rust_primitives.Hax.box_new (let list = [g_pow_xi_yi_vi] in
+                  FStar.Pervasives.assert_norm (Prims.eq2 (List.Tot.length list) 1);
+                  Rust_primitives.Hax.array_of_list 1 list)
+              <:
+              Alloc.Boxed.t_Box (t_Array v_G (sz 1)) Alloc.Alloc.t_Global)
+          <:
+          Alloc.Boxed.t_Box (t_Slice v_G) Alloc.Alloc.t_Global)
+      <:
+      Alloc.Vec.t_Vec v_G Alloc.Alloc.t_Global)
+
+let compute_group_element_for_vote
+      (#v_G: Type0)
+      (#[FStar.Tactics.Typeclasses.tcresolve ()] i1: Hacspec_ovn.Ovn_traits.t_Group v_G)
+      (xi: i1.f_Z)
+      (vote: bool)
+      (g_pow_yi: v_G)
+    : v_G =
+  Hacspec_ovn.Ovn_traits.f_prod #v_G
+    #FStar.Tactics.Typeclasses.solve
+    (Hacspec_ovn.Ovn_traits.f_pow #v_G #FStar.Tactics.Typeclasses.solve g_pow_yi xi <: v_G)
+    (Hacspec_ovn.Ovn_traits.f_g_pow #v_G
+        #FStar.Tactics.Typeclasses.solve
+        (if vote
+          then
+            Hacspec_ovn.Ovn_traits.f_field_one #i1.f_Z #FStar.Tactics.Typeclasses.solve () <: i1.f_Z
+          else
+            Hacspec_ovn.Ovn_traits.f_field_zero #i1.f_Z #FStar.Tactics.Typeclasses.solve ()
+            <:
+            i1.f_Z)
+      <:
+      v_G)
+
+let div
+      (#v_G: Type0)
+      (#[FStar.Tactics.Typeclasses.tcresolve ()] i1: Hacspec_ovn.Ovn_traits.t_Group v_G)
+      (x y: v_G)
+    : v_G =
+  Hacspec_ovn.Ovn_traits.f_prod #v_G
+    #FStar.Tactics.Typeclasses.solve
+    x
+    (Hacspec_ovn.Ovn_traits.f_group_inv #v_G #FStar.Tactics.Typeclasses.solve y <: v_G)
+
+let compute_g_pow_yi
+      (#v_G: Type0)
+      (n: usize)
+      (#[FStar.Tactics.Typeclasses.tcresolve ()] i1: Hacspec_ovn.Ovn_traits.t_Group v_G)
+      (i: usize)
+      (xis: t_Array v_G n)
+    : v_G =
+  let prod1:v_G = Hacspec_ovn.Ovn_traits.f_group_one #v_G #FStar.Tactics.Typeclasses.solve () in
+  let prod1:v_G =
+    Rust_primitives.Hax.Folds.fold_range (sz 0)
+      i
+      (fun prod1 temp_1_ ->
+          let prod1:v_G = prod1 in
+          let _:usize = temp_1_ in
+          true)
+      prod1
+      (fun prod1 j ->
+          let prod1:v_G = prod1 in
+          let j:usize = j in
+          Hacspec_ovn.Ovn_traits.f_prod #v_G
+            #FStar.Tactics.Typeclasses.solve
+            prod1
+            (xis.[ j ] <: v_G)
+          <:
+          v_G)
+  in
+  let prod2:v_G = Hacspec_ovn.Ovn_traits.f_group_one #v_G #FStar.Tactics.Typeclasses.solve () in
+  let prod2:v_G =
+    Rust_primitives.Hax.Folds.fold_range (i +! sz 1 <: usize)
+      n
+      (fun prod2 temp_1_ ->
+          let prod2:v_G = prod2 in
+          let _:usize = temp_1_ in
+          true)
+      prod2
+      (fun prod2 j ->
+          let prod2:v_G = prod2 in
+          let j:usize = j in
+          Hacspec_ovn.Ovn_traits.f_prod #v_G
+            #FStar.Tactics.Typeclasses.solve
+            prod2
+            (xis.[ j ] <: v_G)
+          <:
+          v_G)
+  in
+  div #v_G prod1 prod2
+
+type t_CastVoteParam (v_Z: Type0) {| i1: Hacspec_ovn.Ovn_traits.t_Field v_Z |} = {
+  f_cvp_i:u32;
+  f_cvp_xi:v_Z;
+  f_cvp_zkp_random_w:v_Z;
+  f_cvp_zkp_random_r:v_Z;
+  f_cvp_zkp_random_d:v_Z;
+  f_cvp_vote:bool
+}
+
+type t_OrZKPCommit (v_G: Type0) {| i1: Hacspec_ovn.Ovn_traits.t_Group v_G |} = {
+  f_or_zkp_x:v_G;
+  f_or_zkp_y:v_G;
+  f_or_zkp_a1:v_G;
+  f_or_zkp_b1:v_G;
+  f_or_zkp_a2:v_G;
+  f_or_zkp_b2:v_G;
+  f_or_zkp_c:i1.f_Z;
+  f_or_zkp_d1:i1.f_Z;
+  f_or_zkp_d2:i1.f_Z;
+  f_or_zkp_r1:i1.f_Z;
+  f_or_zkp_r2:i1.f_Z
+}
+
+type t_RegisterParam (v_Z: Type0) {| i1: Hacspec_ovn.Ovn_traits.t_Field v_Z |} = {
+  f_rp_i:u32;
+  f_rp_xi:v_Z;
+  f_rp_zkp_random:v_Z
+}
+
+type t_SchnorrZKPCommit (v_G: Type0) {| i1: Hacspec_ovn.Ovn_traits.t_Group v_G |} = {
+  f_schnorr_zkp_u:v_G;
+  f_schnorr_zkp_c:i1.f_Z;
+  f_schnorr_zkp_z:i1.f_Z
+}
+
+(** Non-interactive Schnorr proof using Fiat-Shamir heuristics (RFC 8235) *)
+let schnorr_zkp
+      (#v_G: Type0)
+      (#[FStar.Tactics.Typeclasses.tcresolve ()] i1: Hacspec_ovn.Ovn_traits.t_Group v_G)
+      (random: i1.f_Z)
+      (h: v_G)
+      (x: i1.f_Z)
+    : t_SchnorrZKPCommit v_G =
+  Rust_primitives.Hax.Control_flow_monad.Mexception.run (let r = random in
+      let u:v_G = Hacspec_ovn.Ovn_traits.f_g_pow #v_G #FStar.Tactics.Typeclasses.solve r in
+      let c =
+        Hacspec_ovn.Ovn_traits.f_hash #v_G
+          #FStar.Tactics.Typeclasses.solve
+          (Alloc.Slice.impl__into_vec #v_G
+              #Alloc.Alloc.t_Global
+              (Rust_primitives.unsize (Rust_primitives.Hax.box_new (let list =
+                          [
+                            Hacspec_ovn.Ovn_traits.f_g #v_G #FStar.Tactics.Typeclasses.solve ()
+                            <:
+                            v_G;
+                            h;
+                            u
+                          ]
+                        in
+                        FStar.Pervasives.assert_norm (Prims.eq2 (List.Tot.length list) 3);
+                        Rust_primitives.Hax.array_of_list 3 list)
+                    <:
+                    Alloc.Boxed.t_Box (t_Array v_G (sz 3)) Alloc.Alloc.t_Global)
+                <:
+                Alloc.Boxed.t_Box (t_Slice v_G) Alloc.Alloc.t_Global)
+            <:
+            Alloc.Vec.t_Vec v_G Alloc.Alloc.t_Global)
+      in
+      let z =
+        Hacspec_ovn.Ovn_traits.f_add #i1.f_Z
+          #FStar.Tactics.Typeclasses.solve
+          r
+          (Hacspec_ovn.Ovn_traits.f_mul #i1.f_Z #FStar.Tactics.Typeclasses.solve c x <: i1.f_Z)
+      in
+      let! hoist9:Rust_primitives.Hax.t_Never =
+        Core.Ops.Control_flow.ControlFlow_Break
+        ({ f_schnorr_zkp_u = u; f_schnorr_zkp_c = c; f_schnorr_zkp_z = z } <: t_SchnorrZKPCommit v_G
+        )
+        <:
+        Core.Ops.Control_flow.t_ControlFlow (t_SchnorrZKPCommit v_G) Rust_primitives.Hax.t_Never
+      in
+      Core.Ops.Control_flow.ControlFlow_Continue (Rust_primitives.Hax.never_to_any hoist9)
+      <:
+      Core.Ops.Control_flow.t_ControlFlow (t_SchnorrZKPCommit v_G) (t_SchnorrZKPCommit v_G))
+
+let schnorr_zkp_validate
+      (#v_G: Type0)
+      (#[FStar.Tactics.Typeclasses.tcresolve ()] i1: Hacspec_ovn.Ovn_traits.t_Group v_G)
+      (h: v_G)
+      (pi: t_SchnorrZKPCommit v_G)
+    : bool =
+  pi.f_schnorr_zkp_c =.
+  (Hacspec_ovn.Ovn_traits.f_hash #v_G
+      #FStar.Tactics.Typeclasses.solve
+      (Alloc.Slice.impl__into_vec #v_G
+          #Alloc.Alloc.t_Global
+          (Rust_primitives.unsize (Rust_primitives.Hax.box_new (let list =
+                      [
+                        Hacspec_ovn.Ovn_traits.f_g #v_G #FStar.Tactics.Typeclasses.solve () <: v_G;
+                        h;
+                        pi.f_schnorr_zkp_u
+                      ]
+                    in
+                    FStar.Pervasives.assert_norm (Prims.eq2 (List.Tot.length list) 3);
+                    Rust_primitives.Hax.array_of_list 3 list)
+                <:
+                Alloc.Boxed.t_Box (t_Array v_G (sz 3)) Alloc.Alloc.t_Global)
+            <:
+            Alloc.Boxed.t_Box (t_Slice v_G) Alloc.Alloc.t_Global)
+        <:
+        Alloc.Vec.t_Vec v_G Alloc.Alloc.t_Global)
+    <:
+    i1.f_Z) &&
+  (Hacspec_ovn.Ovn_traits.f_g_pow #v_G #FStar.Tactics.Typeclasses.solve pi.f_schnorr_zkp_z <: v_G) =.
+  (Hacspec_ovn.Ovn_traits.f_prod #v_G
+      #FStar.Tactics.Typeclasses.solve
+      pi.f_schnorr_zkp_u
+      (Hacspec_ovn.Ovn_traits.f_pow #v_G #FStar.Tactics.Typeclasses.solve h pi.f_schnorr_zkp_c
+        <:
+        v_G)
+    <:
+    v_G)
+
+(** Cramer, Damgård and Schoenmakers (CDS) technique *)
+let zkp_one_out_of_two
+      (#v_G: Type0)
+      (#[FStar.Tactics.Typeclasses.tcresolve ()] i1: Hacspec_ovn.Ovn_traits.t_Group v_G)
+      (random_w random_r random_d: i1.f_Z)
+      (h: v_G)
+      (xi: i1.f_Z)
+      (vi: bool)
+    : t_OrZKPCommit v_G =
+  let w = random_w in
+  if vi
+  then
+    let r1 = random_r in
+    let d1 = random_d in
+    let x:v_G = Hacspec_ovn.Ovn_traits.f_g_pow #v_G #FStar.Tactics.Typeclasses.solve xi in
+    let y:v_G =
+      Hacspec_ovn.Ovn_traits.f_prod #v_G
+        #FStar.Tactics.Typeclasses.solve
+        (Hacspec_ovn.Ovn_traits.f_pow #v_G #FStar.Tactics.Typeclasses.solve h xi <: v_G)
+        (Hacspec_ovn.Ovn_traits.f_g #v_G #FStar.Tactics.Typeclasses.solve () <: v_G)
+    in
+    let a1:v_G =
+      Hacspec_ovn.Ovn_traits.f_prod #v_G
+        #FStar.Tactics.Typeclasses.solve
+        (Hacspec_ovn.Ovn_traits.f_g_pow #v_G #FStar.Tactics.Typeclasses.solve r1 <: v_G)
+        (Hacspec_ovn.Ovn_traits.f_pow #v_G #FStar.Tactics.Typeclasses.solve x d1 <: v_G)
+    in
+    let b1:v_G =
+      Hacspec_ovn.Ovn_traits.f_prod #v_G
+        #FStar.Tactics.Typeclasses.solve
+        (Hacspec_ovn.Ovn_traits.f_pow #v_G #FStar.Tactics.Typeclasses.solve h r1 <: v_G)
+        (Hacspec_ovn.Ovn_traits.f_pow #v_G #FStar.Tactics.Typeclasses.solve y d1 <: v_G)
+    in
+    let a2:v_G = Hacspec_ovn.Ovn_traits.f_g_pow #v_G #FStar.Tactics.Typeclasses.solve w in
+    let b2:v_G = Hacspec_ovn.Ovn_traits.f_pow #v_G #FStar.Tactics.Typeclasses.solve h w in
+    let c =
+      Hacspec_ovn.Ovn_traits.f_hash #v_G
+        #FStar.Tactics.Typeclasses.solve
+        (Alloc.Slice.impl__into_vec #v_G
+            #Alloc.Alloc.t_Global
+            (Rust_primitives.unsize (Rust_primitives.Hax.box_new (let list =
+                        [x; y; a1; b1; a2; b2]
+                      in
+                      FStar.Pervasives.assert_norm (Prims.eq2 (List.Tot.length list) 6);
+                      Rust_primitives.Hax.array_of_list 6 list)
+                  <:
+                  Alloc.Boxed.t_Box (t_Array v_G (sz 6)) Alloc.Alloc.t_Global)
+              <:
+              Alloc.Boxed.t_Box (t_Slice v_G) Alloc.Alloc.t_Global)
+          <:
+          Alloc.Vec.t_Vec v_G Alloc.Alloc.t_Global)
+    in
+    let d2 = sub #i1.f_Z c d1 in
+    let r2 =
+      sub #i1.f_Z
+        w
+        (Hacspec_ovn.Ovn_traits.f_mul #i1.f_Z #FStar.Tactics.Typeclasses.solve xi d2 <: i1.f_Z)
+    in
+    {
+      f_or_zkp_x = x;
+      f_or_zkp_y = y;
+      f_or_zkp_a1 = a1;
+      f_or_zkp_b1 = b1;
+      f_or_zkp_a2 = a2;
+      f_or_zkp_b2 = b2;
+      f_or_zkp_c = c;
+      f_or_zkp_d1 = d1;
+      f_or_zkp_d2 = d2;
+      f_or_zkp_r1 = r1;
+      f_or_zkp_r2 = r2
+    }
+    <:
+    t_OrZKPCommit v_G
+  else
+    let r2 = random_r in
+    let d2 = random_d in
+    let x:v_G = Hacspec_ovn.Ovn_traits.f_g_pow #v_G #FStar.Tactics.Typeclasses.solve xi in
+    let y:v_G = Hacspec_ovn.Ovn_traits.f_pow #v_G #FStar.Tactics.Typeclasses.solve h xi in
+    let a1:v_G = Hacspec_ovn.Ovn_traits.f_g_pow #v_G #FStar.Tactics.Typeclasses.solve w in
+    let b1:v_G = Hacspec_ovn.Ovn_traits.f_pow #v_G #FStar.Tactics.Typeclasses.solve h w in
+    let a2:v_G =
+      Hacspec_ovn.Ovn_traits.f_prod #v_G
+        #FStar.Tactics.Typeclasses.solve
+        (Hacspec_ovn.Ovn_traits.f_g_pow #v_G #FStar.Tactics.Typeclasses.solve r2 <: v_G)
+        (Hacspec_ovn.Ovn_traits.f_pow #v_G #FStar.Tactics.Typeclasses.solve x d2 <: v_G)
+    in
+    let b2:v_G =
+      Hacspec_ovn.Ovn_traits.f_prod #v_G
+        #FStar.Tactics.Typeclasses.solve
+        (Hacspec_ovn.Ovn_traits.f_pow #v_G #FStar.Tactics.Typeclasses.solve h r2 <: v_G)
+        (Hacspec_ovn.Ovn_traits.f_pow #v_G
+            #FStar.Tactics.Typeclasses.solve
+            (div #v_G y (Hacspec_ovn.Ovn_traits.f_g #v_G #FStar.Tactics.Typeclasses.solve () <: v_G)
+              <:
+              v_G)
+            d2
+          <:
+          v_G)
+    in
+    let c =
+      Hacspec_ovn.Ovn_traits.f_hash #v_G
+        #FStar.Tactics.Typeclasses.solve
+        (Alloc.Slice.impl__into_vec #v_G
+            #Alloc.Alloc.t_Global
+            (Rust_primitives.unsize (Rust_primitives.Hax.box_new (let list =
+                        [x; y; a1; b1; a2; b2]
+                      in
+                      FStar.Pervasives.assert_norm (Prims.eq2 (List.Tot.length list) 6);
+                      Rust_primitives.Hax.array_of_list 6 list)
+                  <:
+                  Alloc.Boxed.t_Box (t_Array v_G (sz 6)) Alloc.Alloc.t_Global)
+              <:
+              Alloc.Boxed.t_Box (t_Slice v_G) Alloc.Alloc.t_Global)
+          <:
+          Alloc.Vec.t_Vec v_G Alloc.Alloc.t_Global)
+    in
+    let d1 = sub #i1.f_Z c d2 in
+    let r1 =
+      sub #i1.f_Z
+        w
+        (Hacspec_ovn.Ovn_traits.f_mul #i1.f_Z #FStar.Tactics.Typeclasses.solve xi d1 <: i1.f_Z)
+    in
+    {
+      f_or_zkp_x = x;
+      f_or_zkp_y = y;
+      f_or_zkp_a1 = a1;
+      f_or_zkp_b1 = b1;
+      f_or_zkp_a2 = a2;
+      f_or_zkp_b2 = b2;
+      f_or_zkp_c = c;
+      f_or_zkp_d1 = d1;
+      f_or_zkp_d2 = d2;
+      f_or_zkp_r1 = r1;
+      f_or_zkp_r2 = r2
+    }
+    <:
+    t_OrZKPCommit v_G
+
+let zkp_one_out_of_two_validate
+      (#v_G: Type0)
+      (#[FStar.Tactics.Typeclasses.tcresolve ()] i1: Hacspec_ovn.Ovn_traits.t_Group v_G)
+      (h: v_G)
+      (zkp: t_OrZKPCommit v_G)
+    : bool =
+  let c =
+    Hacspec_ovn.Ovn_traits.f_hash #v_G
+      #FStar.Tactics.Typeclasses.solve
+      (Alloc.Slice.impl__into_vec #v_G
+          #Alloc.Alloc.t_Global
+          (Rust_primitives.unsize (Rust_primitives.Hax.box_new (let list =
+                      [
+                        zkp.f_or_zkp_x;
+                        zkp.f_or_zkp_y;
+                        zkp.f_or_zkp_a1;
+                        zkp.f_or_zkp_b1;
+                        zkp.f_or_zkp_a2;
+                        zkp.f_or_zkp_b2
+                      ]
+                    in
+                    FStar.Pervasives.assert_norm (Prims.eq2 (List.Tot.length list) 6);
+                    Rust_primitives.Hax.array_of_list 6 list)
+                <:
+                Alloc.Boxed.t_Box (t_Array v_G (sz 6)) Alloc.Alloc.t_Global)
+            <:
+            Alloc.Boxed.t_Box (t_Slice v_G) Alloc.Alloc.t_Global)
+        <:
+        Alloc.Vec.t_Vec v_G Alloc.Alloc.t_Global)
+  in
+  c =.
+  (Hacspec_ovn.Ovn_traits.f_add #i1.f_Z
+      #FStar.Tactics.Typeclasses.solve
+      zkp.f_or_zkp_d1
+      zkp.f_or_zkp_d2
+    <:
+    i1.f_Z) &&
+  zkp.f_or_zkp_a1 =.
+  (Hacspec_ovn.Ovn_traits.f_prod #v_G
+      #FStar.Tactics.Typeclasses.solve
+      (Hacspec_ovn.Ovn_traits.f_g_pow #v_G #FStar.Tactics.Typeclasses.solve zkp.f_or_zkp_r1 <: v_G)
+      (Hacspec_ovn.Ovn_traits.f_pow #v_G
+          #FStar.Tactics.Typeclasses.solve
+          zkp.f_or_zkp_x
+          zkp.f_or_zkp_d1
+        <:
+        v_G)
+    <:
+    v_G) &&
+  zkp.f_or_zkp_b1 =.
+  (Hacspec_ovn.Ovn_traits.f_prod #v_G
+      #FStar.Tactics.Typeclasses.solve
+      (Hacspec_ovn.Ovn_traits.f_pow #v_G #FStar.Tactics.Typeclasses.solve h zkp.f_or_zkp_r1 <: v_G)
+      (Hacspec_ovn.Ovn_traits.f_pow #v_G
+          #FStar.Tactics.Typeclasses.solve
+          zkp.f_or_zkp_y
+          zkp.f_or_zkp_d1
+        <:
+        v_G)
+    <:
+    v_G) &&
+  zkp.f_or_zkp_a2 =.
+  (Hacspec_ovn.Ovn_traits.f_prod #v_G
+      #FStar.Tactics.Typeclasses.solve
+      (Hacspec_ovn.Ovn_traits.f_g_pow #v_G #FStar.Tactics.Typeclasses.solve zkp.f_or_zkp_r2 <: v_G)
+      (Hacspec_ovn.Ovn_traits.f_pow #v_G
+          #FStar.Tactics.Typeclasses.solve
+          zkp.f_or_zkp_x
+          zkp.f_or_zkp_d2
+        <:
+        v_G)
+    <:
+    v_G) &&
+  zkp.f_or_zkp_b2 =.
+  (Hacspec_ovn.Ovn_traits.f_prod #v_G
+      #FStar.Tactics.Typeclasses.solve
+      (Hacspec_ovn.Ovn_traits.f_pow #v_G #FStar.Tactics.Typeclasses.solve h zkp.f_or_zkp_r2 <: v_G)
+      (Hacspec_ovn.Ovn_traits.f_pow #v_G
+          #FStar.Tactics.Typeclasses.solve
+          (div #v_G
+              zkp.f_or_zkp_y
+              (Hacspec_ovn.Ovn_traits.f_g #v_G #FStar.Tactics.Typeclasses.solve () <: v_G)
+            <:
+            v_G)
+          zkp.f_or_zkp_d2
+        <:
+        v_G)
+    <:
+    v_G)
+
+type t_OvnContractState (v_G: Type0) (n: usize) {| i1: Hacspec_ovn.Ovn_traits.t_Group v_G |} = {
+  f_g_pow_xis:t_Array v_G n;
+  f_zkp_xis:t_Array (t_SchnorrZKPCommit v_G) n;
+  f_commit_vis:t_Array i1.f_Z n;
+  f_g_pow_xi_yi_vis:t_Array v_G n;
+  f_zkp_vis:t_Array (t_OrZKPCommit v_G) n;
+  f_tally:u32;
+  f_round1:t_Array bool n
+}
+
+(** Primary function in round 2, also opens commitment *)
+let cast_vote
+      (#v_G: Type0)
+      (n: usize)
+      (#v_A #impl_574521470_: Type0)
+      (#[FStar.Tactics.Typeclasses.tcresolve ()] i3: Hacspec_ovn.Ovn_traits.t_Group v_G)
+      (#[FStar.Tactics.Typeclasses.tcresolve ()]
+          i4:
+          Hacspec_concordium.Concordium_traits.t_HasActions v_A)
+      (#[FStar.Tactics.Typeclasses.tcresolve ()]
+          i5:
+          Hacspec_concordium.Concordium_traits.t_HasReceiveContext impl_574521470_ Prims.unit)
+      (ctx: impl_574521470_)
+      (state: t_OvnContractState v_G n)
+    : Core.Result.t_Result (v_A & t_OvnContractState v_G n)
+      Concordium_contracts_common.Types.t_ParseError =
+  let _, out:(_ &
+    Core.Result.t_Result (t_CastVoteParam i3.f_Z) Concordium_contracts_common.Types.t_ParseError) =
+    Concordium_contracts_common.Traits.f_get #_
+      #(t_CastVoteParam i3.f_Z)
+      #FStar.Tactics.Typeclasses.solve
+      (Hacspec_concordium.Concordium_traits.f_parameter_cursor #impl_574521470_
+          #FStar.Tactics.Typeclasses.solve
+          ctx
+        <:
+        _)
+  in
+  match out with
+  | Core.Result.Result_Ok (params: t_CastVoteParam i3.f_Z) ->
+    let g_pow_yi:v_G =
+      compute_g_pow_yi #v_G n (cast (params.f_cvp_i <: u32) <: usize) state.f_g_pow_xis
+    in
+    let g_pow_xi_yi_vi:v_G =
+      compute_group_element_for_vote #v_G params.f_cvp_xi params.f_cvp_vote g_pow_yi
+    in
+    let zkp_vi:t_OrZKPCommit v_G =
+      zkp_one_out_of_two #v_G
+        params.f_cvp_zkp_random_w
+        params.f_cvp_zkp_random_r
+        params.f_cvp_zkp_random_d
+        g_pow_yi
+        params.f_cvp_xi
+        params.f_cvp_vote
+    in
+    let cast_vote_state_ret:t_OvnContractState v_G n =
+      Core.Clone.f_clone #(t_OvnContractState v_G n) #FStar.Tactics.Typeclasses.solve state
+    in
+    let cast_vote_state_ret:t_OvnContractState v_G n =
+      {
+        cast_vote_state_ret with
+        f_g_pow_xi_yi_vis
+        =
+        Rust_primitives.Hax.Monomorphized_update_at.update_at_usize cast_vote_state_ret
+            .f_g_pow_xi_yi_vis
+          (cast (params.f_cvp_i <: u32) <: usize)
+          g_pow_xi_yi_vi
+      }
+      <:
+      t_OvnContractState v_G n
+    in
+    let cast_vote_state_ret:t_OvnContractState v_G n =
+      {
+        cast_vote_state_ret with
+        f_zkp_vis
+        =
+        Rust_primitives.Hax.Monomorphized_update_at.update_at_usize cast_vote_state_ret.f_zkp_vis
+          (cast (params.f_cvp_i <: u32) <: usize)
+          zkp_vi
+      }
+      <:
+      t_OvnContractState v_G n
+    in
+    Core.Result.Result_Ok
+    (Hacspec_concordium.Concordium_traits.f_accept #v_A #FStar.Tactics.Typeclasses.solve (),
+      cast_vote_state_ret
+      <:
+      (v_A & t_OvnContractState v_G n))
+    <:
+    Core.Result.t_Result (v_A & t_OvnContractState v_G n)
+      Concordium_contracts_common.Types.t_ParseError
+  | Core.Result.Result_Err err ->
+    Core.Result.Result_Err err
+    <:
+    Core.Result.t_Result (v_A & t_OvnContractState v_G n)
+      Concordium_contracts_common.Types.t_ParseError
+
+(** Commitment before round 2 *)
+let commit_to_vote
+      (#v_G: Type0)
+      (n: usize)
+      (#v_A #impl_574521470_: Type0)
+      (#[FStar.Tactics.Typeclasses.tcresolve ()] i3: Hacspec_ovn.Ovn_traits.t_Group v_G)
+      (#[FStar.Tactics.Typeclasses.tcresolve ()]
+          i4:
+          Hacspec_concordium.Concordium_traits.t_HasActions v_A)
+      (#[FStar.Tactics.Typeclasses.tcresolve ()]
+          i5:
+          Hacspec_concordium.Concordium_traits.t_HasReceiveContext impl_574521470_ Prims.unit)
+      (ctx: impl_574521470_)
+      (state: t_OvnContractState v_G n)
+    : Core.Result.t_Result (v_A & t_OvnContractState v_G n)
+      Concordium_contracts_common.Types.t_ParseError =
+  let _, out:(_ &
+    Core.Result.t_Result (t_CastVoteParam i3.f_Z) Concordium_contracts_common.Types.t_ParseError) =
+    Concordium_contracts_common.Traits.f_get #_
+      #(t_CastVoteParam i3.f_Z)
+      #FStar.Tactics.Typeclasses.solve
+      (Hacspec_concordium.Concordium_traits.f_parameter_cursor #impl_574521470_
+          #FStar.Tactics.Typeclasses.solve
+          ctx
+        <:
+        _)
+  in
+  match out with
+  | Core.Result.Result_Ok (params: t_CastVoteParam i3.f_Z) ->
+    let _:Prims.unit =
+      Rust_primitives.Hax.failure "(FunctionalizeLoops) something is not implemented yet.\nLoop without mutation?"
+        "{\n        for i in (core::iter::traits::collect::f_into_iter(core::ops::range::Range {\n            f_start: 0,\n            f_end: n,\n        })) {\n            (if BinOp::Ast\n                .Or(\n                    core::ops::bit::Not::not(\n                        hacspec_ovn::ovn_group::schnorr_zkp_validate::<\n                            G,\n                        >(\n                            core::ops::index::Index::index(\n                                proj_hacspec_ovn::ovn_group::f_g_pow_xis(state),\n                                i,\n                            ),\n                            core::ops::index::Index::index(\n                                proj_hacspec_ovn::ovn_group::f_zkp_xis(state),\n                                i,\n                            ),\n                        ),\n                    ),\n                    core::ops::bit::Not::not(\n                        core::ops::index::Index::index(\n                            proj_hacspec_ovn::ovn_group::f_round1(state),\n                            i,\n                        ),\n                    ),\n                )\n            {\n                {\n                    #[note(\n                        \"rhs.typ=core::ops::control_flow::t_ControlFlow<core::result::t_Result<tuple2<A, hacspec_ovn::ovn_group::t_OvnContractState<G, generic_value!(todo)>>, concordium_contracts_common::types::t_ParseError>, rust_primitives::hax::t_Never>\"\n                    )]\n                    #[monadic_let(\n                        MException<core::result::t_Result<tuple2<A,\n                        hacspec_ovn::ovn_group::t_OvnContractState<G,\n                        generic_value!(todo)>>,\n                        concordium_contracts_common::types::t_ParseError>>\n                    )]\n                    let hoist12: rust_primitives::hax::t_Never = {\n                        core::ops::control_flow::ControlFlow_Break(\n                            core::result::Result_Err(\n                                concordium_contracts_common::types::ParseError(),\n                            ),\n                        )\n                    };\n                    core::ops::control_flow::ControlFlow_Continue(\n                        rust_primitives::hax::never_to_any(hoist12),\n                    )\n                }\n            } else {\n                core::ops::control_flow::ControlFlow_Continue(Tuple0)\n            })\n        }\n    }"
+
+    in
+    let g_pow_yi:v_G =
+      compute_g_pow_yi #v_G n (cast (params.f_cvp_i <: u32) <: usize) state.f_g_pow_xis
+    in
+    let g_pow_xi_yi_vi:v_G =
+      compute_group_element_for_vote #v_G params.f_cvp_xi params.f_cvp_vote g_pow_yi
+    in
+    let commit_vi = commit_to #v_G g_pow_xi_yi_vi in
+    let commit_to_vote_state_ret:t_OvnContractState v_G n =
+      Core.Clone.f_clone #(t_OvnContractState v_G n) #FStar.Tactics.Typeclasses.solve state
+    in
+    let commit_to_vote_state_ret:t_OvnContractState v_G n =
+      {
+        commit_to_vote_state_ret with
+        f_commit_vis
+        =
+        Rust_primitives.Hax.Monomorphized_update_at.update_at_usize commit_to_vote_state_ret
+            .f_commit_vis
+          (cast (params.f_cvp_i <: u32) <: usize)
+          commit_vi
+      }
+      <:
+      t_OvnContractState v_G n
+    in
+    Core.Result.Result_Ok
+    (Hacspec_concordium.Concordium_traits.f_accept #v_A #FStar.Tactics.Typeclasses.solve (),
+      commit_to_vote_state_ret
+      <:
+      (v_A & t_OvnContractState v_G n))
+    <:
+    Core.Result.t_Result (v_A & t_OvnContractState v_G n)
+      Concordium_contracts_common.Types.t_ParseError
+  | Core.Result.Result_Err err ->
+    Core.Result.Result_Err err
+    <:
+    Core.Result.t_Result (v_A & t_OvnContractState v_G n)
+      Concordium_contracts_common.Types.t_ParseError
+
+let init_ovn_contract
+      (#v_G: Type0)
+      (n: usize)
+      (#[FStar.Tactics.Typeclasses.tcresolve ()] i1: Hacspec_ovn.Ovn_traits.t_Group v_G)
+      (_: Prims.unit)
+    : Core.Result.t_Result (t_OvnContractState v_G n) Hacspec_concordium.Concordium_types.t_Reject =
+  Core.Result.Result_Ok
+  ({
+      f_g_pow_xis
+      =
+      Rust_primitives.Hax.repeat (Hacspec_ovn.Ovn_traits.f_group_one #v_G
+            #FStar.Tactics.Typeclasses.solve
+            ()
+          <:
+          v_G)
+        n;
+      f_zkp_xis
+      =
+      Rust_primitives.Hax.repeat ({
+            f_schnorr_zkp_u
+            =
+            Hacspec_ovn.Ovn_traits.f_group_one #v_G #FStar.Tactics.Typeclasses.solve () <: v_G;
+            f_schnorr_zkp_z
+            =
+            Hacspec_ovn.Ovn_traits.f_field_zero #i1.f_Z #FStar.Tactics.Typeclasses.solve ()
+            <:
+            i1.f_Z;
+            f_schnorr_zkp_c
+            =
+            Hacspec_ovn.Ovn_traits.f_field_zero #i1.f_Z #FStar.Tactics.Typeclasses.solve ()
+            <:
+            i1.f_Z
+          }
+          <:
+          t_SchnorrZKPCommit v_G)
+        n;
+      f_commit_vis
+      =
+      Rust_primitives.Hax.repeat (Hacspec_ovn.Ovn_traits.f_field_zero #i1.f_Z
+            #FStar.Tactics.Typeclasses.solve
+            ()
+          <:
+          i1.f_Z)
+        n;
+      f_g_pow_xi_yi_vis
+      =
+      Rust_primitives.Hax.repeat (Hacspec_ovn.Ovn_traits.f_group_one #v_G
+            #FStar.Tactics.Typeclasses.solve
+            ()
+          <:
+          v_G)
+        n;
+      f_zkp_vis
+      =
+      Rust_primitives.Hax.repeat ({
+            f_or_zkp_x
+            =
+            Hacspec_ovn.Ovn_traits.f_group_one #v_G #FStar.Tactics.Typeclasses.solve () <: v_G;
+            f_or_zkp_y
+            =
+            Hacspec_ovn.Ovn_traits.f_group_one #v_G #FStar.Tactics.Typeclasses.solve () <: v_G;
+            f_or_zkp_a1
+            =
+            Hacspec_ovn.Ovn_traits.f_group_one #v_G #FStar.Tactics.Typeclasses.solve () <: v_G;
+            f_or_zkp_b1
+            =
+            Hacspec_ovn.Ovn_traits.f_group_one #v_G #FStar.Tactics.Typeclasses.solve () <: v_G;
+            f_or_zkp_a2
+            =
+            Hacspec_ovn.Ovn_traits.f_group_one #v_G #FStar.Tactics.Typeclasses.solve () <: v_G;
+            f_or_zkp_b2
+            =
+            Hacspec_ovn.Ovn_traits.f_group_one #v_G #FStar.Tactics.Typeclasses.solve () <: v_G;
+            f_or_zkp_c
+            =
+            Hacspec_ovn.Ovn_traits.f_field_zero #i1.f_Z #FStar.Tactics.Typeclasses.solve ()
+            <:
+            i1.f_Z;
+            f_or_zkp_d1
+            =
+            Hacspec_ovn.Ovn_traits.f_field_zero #i1.f_Z #FStar.Tactics.Typeclasses.solve ()
+            <:
+            i1.f_Z;
+            f_or_zkp_d2
+            =
+            Hacspec_ovn.Ovn_traits.f_field_zero #i1.f_Z #FStar.Tactics.Typeclasses.solve ()
+            <:
+            i1.f_Z;
+            f_or_zkp_r1
+            =
+            Hacspec_ovn.Ovn_traits.f_field_zero #i1.f_Z #FStar.Tactics.Typeclasses.solve ()
+            <:
+            i1.f_Z;
+            f_or_zkp_r2
+            =
+            Hacspec_ovn.Ovn_traits.f_field_zero #i1.f_Z #FStar.Tactics.Typeclasses.solve ()
+            <:
+            i1.f_Z
+          }
+          <:
+          t_OrZKPCommit v_G)
+        n;
+      f_tally = 0ul;
+      f_round1 = Rust_primitives.Hax.repeat false n
+    }
+    <:
+    t_OvnContractState v_G n)
+  <:
+  Core.Result.t_Result (t_OvnContractState v_G n) Hacspec_concordium.Concordium_types.t_Reject
+
+(** Primary function in round 1 *)
+let register_vote
+      (#v_G: Type0)
+      (n: usize)
+      (#v_A #impl_574521470_: Type0)
+      (#[FStar.Tactics.Typeclasses.tcresolve ()] i3: Hacspec_ovn.Ovn_traits.t_Group v_G)
+      (#[FStar.Tactics.Typeclasses.tcresolve ()]
+          i4:
+          Hacspec_concordium.Concordium_traits.t_HasActions v_A)
+      (#[FStar.Tactics.Typeclasses.tcresolve ()]
+          i5:
+          Hacspec_concordium.Concordium_traits.t_HasReceiveContext impl_574521470_ Prims.unit)
+      (ctx: impl_574521470_)
+      (state: t_OvnContractState v_G n)
+    : Core.Result.t_Result (v_A & t_OvnContractState v_G n)
+      Concordium_contracts_common.Types.t_ParseError =
+  let _, out:(_ &
+    Core.Result.t_Result (t_RegisterParam i3.f_Z) Concordium_contracts_common.Types.t_ParseError) =
+    Concordium_contracts_common.Traits.f_get #_
+      #(t_RegisterParam i3.f_Z)
+      #FStar.Tactics.Typeclasses.solve
+      (Hacspec_concordium.Concordium_traits.f_parameter_cursor #impl_574521470_
+          #FStar.Tactics.Typeclasses.solve
+          ctx
+        <:
+        _)
+  in
+  match out with
+  | Core.Result.Result_Ok (params: t_RegisterParam i3.f_Z) ->
+    let g_pow_xi:v_G =
+      Hacspec_ovn.Ovn_traits.f_g_pow #v_G #FStar.Tactics.Typeclasses.solve params.f_rp_xi
+    in
+    let zkp_xi:t_SchnorrZKPCommit v_G =
+      schnorr_zkp #v_G params.f_rp_zkp_random g_pow_xi params.f_rp_xi
+    in
+    let register_vote_state_ret:t_OvnContractState v_G n =
+      Core.Clone.f_clone #(t_OvnContractState v_G n) #FStar.Tactics.Typeclasses.solve state
+    in
+    let register_vote_state_ret:t_OvnContractState v_G n =
+      {
+        register_vote_state_ret with
+        f_g_pow_xis
+        =
+        Rust_primitives.Hax.Monomorphized_update_at.update_at_usize register_vote_state_ret
+            .f_g_pow_xis
+          (cast (params.f_rp_i <: u32) <: usize)
+          g_pow_xi
+      }
+      <:
+      t_OvnContractState v_G n
+    in
+    let register_vote_state_ret:t_OvnContractState v_G n =
+      {
+        register_vote_state_ret with
+        f_zkp_xis
+        =
+        Rust_primitives.Hax.Monomorphized_update_at.update_at_usize register_vote_state_ret
+            .f_zkp_xis
+          (cast (params.f_rp_i <: u32) <: usize)
+          zkp_xi
+      }
+      <:
+      t_OvnContractState v_G n
+    in
+    let register_vote_state_ret:t_OvnContractState v_G n =
+      {
+        register_vote_state_ret with
+        f_round1
+        =
+        Rust_primitives.Hax.Monomorphized_update_at.update_at_usize register_vote_state_ret.f_round1
+          (cast (params.f_rp_i <: u32) <: usize)
+          true
+      }
+      <:
+      t_OvnContractState v_G n
+    in
+    Core.Result.Result_Ok
+    (Hacspec_concordium.Concordium_traits.f_accept #v_A #FStar.Tactics.Typeclasses.solve (),
+      register_vote_state_ret
+      <:
+      (v_A & t_OvnContractState v_G n))
+    <:
+    Core.Result.t_Result (v_A & t_OvnContractState v_G n)
+      Concordium_contracts_common.Types.t_ParseError
+  | Core.Result.Result_Err err ->
+    Core.Result.Result_Err err
+    <:
+    Core.Result.t_Result (v_A & t_OvnContractState v_G n)
+      Concordium_contracts_common.Types.t_ParseError
+
+(** Anyone can tally the votes *)
+let tally_votes
+      (#v_G: Type0)
+      (n: usize)
+      (#v_A: Type0)
+      (#impl_574521470_: Type0)
+      (#[FStar.Tactics.Typeclasses.tcresolve ()] i3: Hacspec_ovn.Ovn_traits.t_Group v_G)
+      (#[FStar.Tactics.Typeclasses.tcresolve ()]
+          i4:
+          Hacspec_concordium.Concordium_traits.t_HasActions v_A)
+      (#[FStar.Tactics.Typeclasses.tcresolve ()]
+          i5:
+          Hacspec_concordium.Concordium_traits.t_HasReceiveContext impl_574521470_ Prims.unit)
+      (_: impl_574521470_)
+      (state: t_OvnContractState v_G n)
+    : Core.Result.t_Result (v_A & t_OvnContractState v_G n)
+      Concordium_contracts_common.Types.t_ParseError =
+  let _:Prims.unit =
+    Rust_primitives.Hax.failure "(FunctionalizeLoops) something is not implemented yet.\nLoop without mutation?"
+      "{\n        for i in (core::iter::traits::collect::f_into_iter(core::ops::range::Range {\n            f_start: 0,\n            f_end: n,\n        })) {\n            {\n                let g_pow_yi: G = {\n                    hacspec_ovn::ovn_group::compute_g_pow_yi::<\n                        G,\n                        generic_value!(todo),\n                    >(i, proj_hacspec_ovn::ovn_group::f_g_pow_xis(state))\n                };\n                {\n                    #[note(\n                        \"rhs.typ=core::ops::control_flow::t_ControlFlow<core::result::t_Result<tuple2<A, hacspec_ovn::ovn_group::t_OvnContractState<G, generic_value!(todo)>>, concordium_contracts_common::types::t_ParseError>, core::ops::control_flow::t_ControlFlow<core::result::t_Result<tuple2<A, hacspec_ovn::ovn_group::t_OvnContractState<G, generic_value!(todo)>>, concordium_contracts_common::types::t_ParseError>, tuple0>>\"\n                    )]\n                    #[monadic_let(\n                        MException<core::result::t_Result<tuple2<A,\n                        hacspec_ovn::ovn_group::t_OvnContractState<G,\n                        generic_value!(todo)>>,\n                        concordium_contracts_common::types::t_ParseError>>\n                    )]\n                    let _: tuple0 = {\n                        core::ops::control_flow::ControlFlow_Continue(\n                            (if core::ops::bit::Not::not(\n                                hacspec_ovn::ovn_group::zkp_one_out_of_two_validate::<\n                                    G,\n                                >(\n                                    g_pow_yi,\n                                    core::ops::index::Index::index(\n                                        proj_hacspec_ovn::ovn_group::f_zkp_vis(state),\n                                        i,\n                                    ),\n                                ),\n                            ) {\n                                {\n                                    #[note(\n                                        \"rhs.typ=core::ops::control_flow::t_ControlFlow<core::result::t_Result<tuple2<A, hacspec_ovn::ovn_group::t_OvnContractState<G, generic_value!(todo)>>, concordium_contracts_common::types::t_ParseError>, rust_primitives::hax::t_Never>\"\n                                    )]\n                                    #[monadic_let(\n                                        MException<core::result::t_Result<tuple2<A,\n                                        hacspec_ovn::ovn_group::t_OvnContractState<G,\n                                        generic_value!(todo)>>,\n                                        concordium_contracts_common::types::t_ParseError>>\n                                    )]\n                                    let hoist13: rust_primitives::hax::t_Never = {\n                                        core::ops::control_flow::ControlFlow_Break(\n                                            core::result::Result_Err(\n                                                concordium_contracts_common::types::ParseError(),\n                                            ),\n                                        )\n                                    };\n                                    core::ops::control_flow::ControlFlow_Continue(\n                                        rust_primitives::hax::never_to_any(hoist13),\n                                    )\n                                }\n                            } else {\n                                core::ops::control_flow::ControlFlow_Continue(Tuple0)\n                            }),\n                        )\n                    };\n                    (if core::ops::bit::Not::not(\n                        hacspec_ovn::ovn_group::check_commitment::<\n                            G,\n                        >(\n                            core::ops::index::Index::index(\n                                proj_hacspec_ovn::ovn_group::f_g_pow_xi_yi_vis(state),\n                                i,\n                            ),\n                            core::ops::index::Index::index(\n                                proj_hacspec_ovn::ovn_group::f_commit_vis(state),\n                                i,\n                            ),\n                        ),\n                    ) {\n                        {\n                            #[note(\n                                \"rhs.typ=core::ops::control_flow::t_ControlFlow<core::result::t_Result<tuple2<A, hacspec_ovn::ovn_group::t_OvnContractState<G, generic_value!(todo)>>, concordium_contracts_common::types::t_ParseError>, rust_primitives::hax::t_Never>\"\n                            )]\n                            #[monadic_let(\n                                MException<core::result::t_Result<tuple2<A,\n                                hacspec_ovn::ovn_group::t_OvnContractState<G,\n                                generic_value!(todo)>>,\n                                concordium_contracts_common::types::t_ParseError>>\n                            )]\n                            let hoist14: rust_primitives::hax::t_Never = {\n                                core::ops::control_flow::ControlFlow_Break(\n                                    core::result::Result_Err(\n                                        concordium_contracts_common::types::ParseError(),\n                                    ),\n                                )\n                            };\n                            core::ops::control_flow::ControlFlow_Continue(\n                                rust_primitives::hax::never_to_any(hoist14),\n                            )\n                        }\n                    } else {\n                        core::ops::control_flow::ControlFlow_Continue(Tuple0)\n                    })\n                }\n            }\n        }\n    }"
+
+  in
+  let vote_result:v_G =
+    Hacspec_ovn.Ovn_traits.f_group_one #v_G #FStar.Tactics.Typeclasses.solve ()
+  in
+  let vote_result:v_G =
+    Core.Iter.Traits.Iterator.f_fold (Core.Iter.Traits.Collect.f_into_iter #(t_Array v_G n)
+          #FStar.Tactics.Typeclasses.solve
+          state.f_g_pow_xi_yi_vis
+        <:
+        Core.Array.Iter.t_IntoIter v_G n)
+      vote_result
+      (fun vote_result g_pow_vote ->
+          let vote_result:v_G = vote_result in
+          let g_pow_vote:v_G = g_pow_vote in
+          Hacspec_ovn.Ovn_traits.f_prod #v_G #FStar.Tactics.Typeclasses.solve vote_result g_pow_vote
+          <:
+          v_G)
+  in
+  let tally:u32 = 0ul in
+  let curr = Hacspec_ovn.Ovn_traits.f_field_zero #i3.f_Z #FStar.Tactics.Typeclasses.solve () in
+  let curr, tally:(i3.f_Z & u32) =
+    Rust_primitives.Hax.Folds.fold_range 0ul
+      (cast (n <: usize) <: u32)
+      (fun temp_0_ temp_1_ ->
+          let curr, tally:(i3.f_Z & u32) = temp_0_ in
+          let _:u32 = temp_1_ in
+          true)
+      (curr, tally <: (i3.f_Z & u32))
+      (fun temp_0_ i ->
+          let curr, tally:(i3.f_Z & u32) = temp_0_ in
+          let i:u32 = i in
+          let tally:u32 =
+            if
+              (Hacspec_ovn.Ovn_traits.f_g_pow #v_G #FStar.Tactics.Typeclasses.solve curr <: v_G) =.
+              vote_result
+            then
+              let tally:u32 = i in
+              tally
+            else tally
+          in
+          let curr =
+            Hacspec_ovn.Ovn_traits.f_add #i3.f_Z
+              #FStar.Tactics.Typeclasses.solve
+              curr
+              (Hacspec_ovn.Ovn_traits.f_field_one #i3.f_Z #FStar.Tactics.Typeclasses.solve ()
+                <:
+                i3.f_Z)
+          in
+          curr, tally <: (i3.f_Z & u32))
+  in
+  let tally_votes_state_ret:t_OvnContractState v_G n =
+    Core.Clone.f_clone #(t_OvnContractState v_G n) #FStar.Tactics.Typeclasses.solve state
+  in
+  let tally_votes_state_ret:t_OvnContractState v_G n =
+    { tally_votes_state_ret with f_tally = tally } <: t_OvnContractState v_G n
+  in
+  Core.Result.Result_Ok
+  (Hacspec_concordium.Concordium_traits.f_accept #v_A #FStar.Tactics.Typeclasses.solve (),
+    tally_votes_state_ret
+    <:
+    (v_A & t_OvnContractState v_G n))
+  <:
+  Core.Result.t_Result (v_A & t_OvnContractState v_G n)
+    Concordium_contracts_common.Types.t_ParseError
