ovn/proofs/fstar/extraction/Hacspec_ovn.Ovn_secp256k1.fst
@@ -1,0 +1,740 @@
+module Hacspec_ovn.Ovn_secp256k1
+#set-options "--fuel 0 --ifuel 1 --z3rlimit 15"
+open Core
+open FStar.Mul
+
+let _ =
+  (* This module has implicit dependencies, here we make them explicit. *)
+  (* The implicit dependencies arise from typeclasses instances. *)
+  let open Concordium_contracts_common.Impls in
+  let open Concordium_contracts_common.Traits in
+  let open Hacspec_bip_340 in
+  let open Hacspec_lib.Seq in
+  let open Hacspec_ovn.Ovn_traits in
+  ()
+
+type t_Group_curve = { f_g_val:Hacspec_bip_340.t_Point }
+
+[@@ FStar.Tactics.Typeclasses.tcinstance]
+let impl_3: Concordium_contracts_common.Traits.t_Deserial t_Group_curve =
+  {
+    f_deserial_pre
+    =
+    (fun
+        (#v_R: Type0)
+        (#[FStar.Tactics.Typeclasses.tcresolve ()]
+          i1:
+          Concordium_contracts_common.Traits.t_Read v_R)
+        (source: v_R)
+        ->
+        true);
+    f_deserial_post
+    =
+    (fun
+        (#v_R: Type0)
+        (#[FStar.Tactics.Typeclasses.tcresolve ()]
+          i1:
+          Concordium_contracts_common.Traits.t_Read v_R)
+        (source: v_R)
+        (out1:
+          (v_R & Core.Result.t_Result t_Group_curve Concordium_contracts_common.Types.t_ParseError))
+        ->
+        true);
+    f_deserial
+    =
+    fun
+      (#v_R: Type0)
+      (#[FStar.Tactics.Typeclasses.tcresolve ()] i1: Concordium_contracts_common.Traits.t_Read v_R)
+      (source: v_R)
+      ->
+      let tmp0, out:(v_R & Core.Result.t_Result bool Concordium_contracts_common.Types.t_ParseError)
+      =
+        Concordium_contracts_common.Traits.f_get #v_R #bool #FStar.Tactics.Typeclasses.solve source
+      in
+      let source:v_R = tmp0 in
+      match out with
+      | Core.Result.Result_Ok (b: bool) ->
+        let source, hax_temp_output:(v_R &
+          Core.Result.t_Result t_Group_curve Concordium_contracts_common.Types.t_ParseError) =
+          if b
+          then
+            let tmp0, out:(v_R &
+              Core.Result.t_Result (Alloc.Vec.t_Vec u8 Alloc.Alloc.t_Global)
+                Concordium_contracts_common.Types.t_ParseError) =
+              Concordium_contracts_common.Traits.f_get #v_R
+                #(Alloc.Vec.t_Vec u8 Alloc.Alloc.t_Global)
+                #FStar.Tactics.Typeclasses.solve
+                source
+            in
+            let source:v_R = tmp0 in
+            match out with
+            | Core.Result.Result_Ok (vx: Alloc.Vec.t_Vec u8 Alloc.Alloc.t_Global) ->
+              let tmp0, out:(v_R &
+                Core.Result.t_Result (Alloc.Vec.t_Vec u8 Alloc.Alloc.t_Global)
+                  Concordium_contracts_common.Types.t_ParseError) =
+                Concordium_contracts_common.Traits.f_get #v_R
+                  #(Alloc.Vec.t_Vec u8 Alloc.Alloc.t_Global)
+                  #FStar.Tactics.Typeclasses.solve
+                  source
+              in
+              let source:v_R = tmp0 in
+              (match out with
+                | Core.Result.Result_Ok (vy: Alloc.Vec.t_Vec u8 Alloc.Alloc.t_Global) ->
+                  source,
+                  (Core.Result.Result_Ok
+                    ({
+                        f_g_val
+                        =
+                        Hacspec_bip_340.Point_Affine
+                        (Hacspec_bip_340.impl__FieldElement__from_public_byte_seq_be #(Hacspec_lib.Seq.t_Seq
+                              u8)
+                            (Hacspec_lib.Seq.impl_52__from_vec #u8 vx <: Hacspec_lib.Seq.t_Seq u8),
+                          Hacspec_bip_340.impl__FieldElement__from_public_byte_seq_be #(Hacspec_lib.Seq.t_Seq
+                              u8)
+                            (Hacspec_lib.Seq.impl_52__from_vec #u8 vy <: Hacspec_lib.Seq.t_Seq u8)
+                          <:
+                          (Hacspec_bip_340.t_FieldElement & Hacspec_bip_340.t_FieldElement))
+                        <:
+                        Hacspec_bip_340.t_Point
+                      }
+                      <:
+                      t_Group_curve)
+                    <:
+                    Core.Result.t_Result t_Group_curve
+                      Concordium_contracts_common.Types.t_ParseError)
+                  <:
+                  (v_R &
+                    Core.Result.t_Result t_Group_curve
+                      Concordium_contracts_common.Types.t_ParseError)
+                | Core.Result.Result_Err err ->
+                  source,
+                  (Core.Ops.Control_flow.ControlFlow_Break
+                    (source,
+                      (Core.Result.Result_Err err
+                        <:
+                        Core.Result.t_Result t_Group_curve
+                          Concordium_contracts_common.Types.t_ParseError)
+                      <:
+                      (v_R &
+                        Core.Result.t_Result t_Group_curve
+                          Concordium_contracts_common.Types.t_ParseError))
+                    <:
+                    Core.Ops.Control_flow.t_ControlFlow
+                      (v_R &
+                        Core.Result.t_Result t_Group_curve
+                          Concordium_contracts_common.Types.t_ParseError)
+                      (Core.Result.t_Result t_Group_curve
+                          Concordium_contracts_common.Types.t_ParseError))
+                  <:
+                  (v_R &
+                    Core.Result.t_Result t_Group_curve
+                      Concordium_contracts_common.Types.t_ParseError))
+            | Core.Result.Result_Err err ->
+              source,
+              (Core.Ops.Control_flow.ControlFlow_Break
+                (source,
+                  (Core.Result.Result_Err err
+                    <:
+                    Core.Result.t_Result t_Group_curve
+                      Concordium_contracts_common.Types.t_ParseError)
+                  <:
+                  (v_R &
+                    Core.Result.t_Result t_Group_curve
+                      Concordium_contracts_common.Types.t_ParseError))
+                <:
+                Core.Ops.Control_flow.t_ControlFlow
+                  (v_R &
+                    Core.Result.t_Result t_Group_curve
+                      Concordium_contracts_common.Types.t_ParseError)
+                  (Core.Result.t_Result t_Group_curve Concordium_contracts_common.Types.t_ParseError
+                  ))
+              <:
+              (v_R &
+                Core.Result.t_Result t_Group_curve Concordium_contracts_common.Types.t_ParseError)
+          else
+            source,
+            (Core.Result.Result_Ok
+              ({ f_g_val = Hacspec_bip_340.Point_AtInfinity <: Hacspec_bip_340.t_Point }
+                <:
+                t_Group_curve)
+              <:
+              Core.Result.t_Result t_Group_curve Concordium_contracts_common.Types.t_ParseError)
+            <:
+            (v_R & Core.Result.t_Result t_Group_curve Concordium_contracts_common.Types.t_ParseError
+            )
+        in
+        source, hax_temp_output
+        <:
+        (v_R & Core.Result.t_Result t_Group_curve Concordium_contracts_common.Types.t_ParseError)
+      | Core.Result.Result_Err err ->
+        source,
+        (Core.Result.Result_Err err
+          <:
+          Core.Result.t_Result t_Group_curve Concordium_contracts_common.Types.t_ParseError)
+        <:
+        (v_R & Core.Result.t_Result t_Group_curve Concordium_contracts_common.Types.t_ParseError)
+  }
+
+[@@ FStar.Tactics.Typeclasses.tcinstance]
+let impl_4: Concordium_contracts_common.Traits.t_Serial t_Group_curve =
+  {
+    f_serial_pre
+    =
+    (fun
+        (#v_W: Type0)
+        (#[FStar.Tactics.Typeclasses.tcresolve ()]
+          i1:
+          Concordium_contracts_common.Traits.t_Write v_W)
+        (self: t_Group_curve)
+        (out: v_W)
+        ->
+        true);
+    f_serial_post
+    =
+    (fun
+        (#v_W: Type0)
+        (#[FStar.Tactics.Typeclasses.tcresolve ()]
+          i1:
+          Concordium_contracts_common.Traits.t_Write v_W)
+        (self: t_Group_curve)
+        (out: v_W)
+        (out2: (v_W & Core.Result.t_Result Prims.unit i1.f_Err))
+        ->
+        true);
+    f_serial
+    =
+    fun
+      (#v_W: Type0)
+      (#[FStar.Tactics.Typeclasses.tcresolve ()] i1: Concordium_contracts_common.Traits.t_Write v_W)
+      (self: t_Group_curve)
+      (out: v_W)
+      ->
+      Rust_primitives.Hax.Control_flow_monad.Mexception.run (let! out:v_W =
+            match self.f_g_val with
+            | Hacspec_bip_340.Point_Affine p ->
+              let tmp0, out1:(v_W & Core.Result.t_Result Prims.unit i1.f_Err) =
+                Concordium_contracts_common.Traits.f_serial #bool
+                  #FStar.Tactics.Typeclasses.solve
+                  #v_W
+                  true
+                  out
+              in
+              let out:v_W = tmp0 in
+              (match out1 with
+                | Core.Result.Result_Ok _ ->
+                  let (vx: Alloc.Vec.t_Vec u8 Alloc.Alloc.t_Global):Alloc.Vec.t_Vec u8
+                    Alloc.Alloc.t_Global =
+                    Alloc.Vec.impl__new #u8 ()
+                  in
+                  let vx:Alloc.Vec.t_Vec u8 Alloc.Alloc.t_Global =
+                    Core.Iter.Traits.Iterator.f_fold (Core.Iter.Traits.Collect.f_into_iter #(t_Slice
+                            u8)
+                          #FStar.Tactics.Typeclasses.solve
+                          (Hacspec_lib.Seq.impl_41__native_slice #u8
+                              (Hacspec_bip_340.impl__FieldElement__to_public_byte_seq_be (Hacspec_bip_340.x
+                                      p
+                                    <:
+                                    Hacspec_bip_340.t_FieldElement)
+                                <:
+                                Hacspec_lib.Seq.t_Seq u8)
+                            <:
+                            t_Slice u8)
+                        <:
+                        Core.Slice.Iter.t_Iter u8)
+                      vx
+                      (fun vx x ->
+                          let vx:Alloc.Vec.t_Vec u8 Alloc.Alloc.t_Global = vx in
+                          let x:u8 = x in
+                          Alloc.Vec.impl_1__push #u8
+                            #Alloc.Alloc.t_Global
+                            vx
+                            (Core.Clone.f_clone #u8 #FStar.Tactics.Typeclasses.solve x <: u8)
+                          <:
+                          Alloc.Vec.t_Vec u8 Alloc.Alloc.t_Global)
+                  in
+                  let tmp0, out1:(v_W & Core.Result.t_Result Prims.unit i1.f_Err) =
+                    Concordium_contracts_common.Traits.f_serial #(Alloc.Vec.t_Vec u8
+                          Alloc.Alloc.t_Global)
+                      #FStar.Tactics.Typeclasses.solve
+                      #v_W
+                      vx
+                      out
+                  in
+                  let out:v_W = tmp0 in
+                  (match out1 with
+                    | Core.Result.Result_Ok _ ->
+                      let (vy: Alloc.Vec.t_Vec u8 Alloc.Alloc.t_Global):Alloc.Vec.t_Vec u8
+                        Alloc.Alloc.t_Global =
+                        Alloc.Vec.impl__new #u8 ()
+                      in
+                      let vy:Alloc.Vec.t_Vec u8 Alloc.Alloc.t_Global =
+                        Core.Iter.Traits.Iterator.f_fold (Core.Iter.Traits.Collect.f_into_iter #(t_Slice
+                                u8)
+                              #FStar.Tactics.Typeclasses.solve
+                              (Hacspec_lib.Seq.impl_41__native_slice #u8
+                                  (Hacspec_bip_340.impl__FieldElement__to_public_byte_seq_be (Hacspec_bip_340.y
+                                          p
+                                        <:
+                                        Hacspec_bip_340.t_FieldElement)
+                                    <:
+                                    Hacspec_lib.Seq.t_Seq u8)
+                                <:
+                                t_Slice u8)
+                            <:
+                            Core.Slice.Iter.t_Iter u8)
+                          vy
+                          (fun vy y ->
+                              let vy:Alloc.Vec.t_Vec u8 Alloc.Alloc.t_Global = vy in
+                              let y:u8 = y in
+                              Alloc.Vec.impl_1__push #u8
+                                #Alloc.Alloc.t_Global
+                                vy
+                                (Core.Clone.f_clone #u8 #FStar.Tactics.Typeclasses.solve y <: u8)
+                              <:
+                              Alloc.Vec.t_Vec u8 Alloc.Alloc.t_Global)
+                      in
+                      let tmp0, out1:(v_W & Core.Result.t_Result Prims.unit i1.f_Err) =
+                        Concordium_contracts_common.Traits.f_serial #(Alloc.Vec.t_Vec u8
+                              Alloc.Alloc.t_Global)
+                          #FStar.Tactics.Typeclasses.solve
+                          #v_W
+                          vy
+                          out
+                      in
+                      let out:v_W = tmp0 in
+                      (match out1 with
+                        | Core.Result.Result_Ok _ ->
+                          Core.Ops.Control_flow.ControlFlow_Continue out
+                          <:
+                          Core.Ops.Control_flow.t_ControlFlow
+                            (v_W & Core.Result.t_Result Prims.unit i1.f_Err) v_W
+                        | Core.Result.Result_Err err ->
+                          let! _:Prims.unit =
+                            Core.Ops.Control_flow.ControlFlow_Break
+                            (out,
+                              (Core.Result.Result_Err err
+                                <:
+                                Core.Result.t_Result Prims.unit i1.f_Err)
+                              <:
+                              (v_W & Core.Result.t_Result Prims.unit i1.f_Err))
+                            <:
+                            Core.Ops.Control_flow.t_ControlFlow
+                              (v_W & Core.Result.t_Result Prims.unit i1.f_Err) Prims.unit
+                          in
+                          Core.Ops.Control_flow.ControlFlow_Continue out
+                          <:
+                          Core.Ops.Control_flow.t_ControlFlow
+                            (v_W & Core.Result.t_Result Prims.unit i1.f_Err) v_W)
+                    | Core.Result.Result_Err err ->
+                      let! _:Prims.unit =
+                        Core.Ops.Control_flow.ControlFlow_Break
+                        (out,
+                          (Core.Result.Result_Err err <: Core.Result.t_Result Prims.unit i1.f_Err)
+                          <:
+                          (v_W & Core.Result.t_Result Prims.unit i1.f_Err))
+                        <:
+                        Core.Ops.Control_flow.t_ControlFlow
+                          (v_W & Core.Result.t_Result Prims.unit i1.f_Err) Prims.unit
+                      in
+                      Core.Ops.Control_flow.ControlFlow_Continue out
+                      <:
+                      Core.Ops.Control_flow.t_ControlFlow
+                        (v_W & Core.Result.t_Result Prims.unit i1.f_Err) v_W)
+                | Core.Result.Result_Err err ->
+                  let! _:Prims.unit =
+                    Core.Ops.Control_flow.ControlFlow_Break
+                    (out, (Core.Result.Result_Err err <: Core.Result.t_Result Prims.unit i1.f_Err)
+                      <:
+                      (v_W & Core.Result.t_Result Prims.unit i1.f_Err))
+                    <:
+                    Core.Ops.Control_flow.t_ControlFlow
+                      (v_W & Core.Result.t_Result Prims.unit i1.f_Err) Prims.unit
+                  in
+                  Core.Ops.Control_flow.ControlFlow_Continue out
+                  <:
+                  Core.Ops.Control_flow.t_ControlFlow
+                    (v_W & Core.Result.t_Result Prims.unit i1.f_Err) v_W)
+            | Hacspec_bip_340.Point_AtInfinity  ->
+              let tmp0, out1:(v_W & Core.Result.t_Result Prims.unit i1.f_Err) =
+                Concordium_contracts_common.Traits.f_serial #bool
+                  #FStar.Tactics.Typeclasses.solve
+                  #v_W
+                  false
+                  out
+              in
+              let out:v_W = tmp0 in
+              match out1 with
+              | Core.Result.Result_Ok _ ->
+                Core.Ops.Control_flow.ControlFlow_Continue out
+                <:
+                Core.Ops.Control_flow.t_ControlFlow (v_W & Core.Result.t_Result Prims.unit i1.f_Err)
+                  v_W
+              | Core.Result.Result_Err err ->
+                let! _:Prims.unit =
+                  Core.Ops.Control_flow.ControlFlow_Break
+                  (out, (Core.Result.Result_Err err <: Core.Result.t_Result Prims.unit i1.f_Err)
+                    <:
+                    (v_W & Core.Result.t_Result Prims.unit i1.f_Err))
+                  <:
+                  Core.Ops.Control_flow.t_ControlFlow
+                    (v_W & Core.Result.t_Result Prims.unit i1.f_Err) Prims.unit
+                in
+                Core.Ops.Control_flow.ControlFlow_Continue out
+                <:
+                Core.Ops.Control_flow.t_ControlFlow (v_W & Core.Result.t_Result Prims.unit i1.f_Err)
+                  v_W
+          in
+          Core.Ops.Control_flow.ControlFlow_Continue
+          (let hax_temp_output:Core.Result.t_Result Prims.unit i1.f_Err =
+              Core.Result.Result_Ok (() <: Prims.unit) <: Core.Result.t_Result Prims.unit i1.f_Err
+            in
+            out, hax_temp_output <: (v_W & Core.Result.t_Result Prims.unit i1.f_Err))
+          <:
+          Core.Ops.Control_flow.t_ControlFlow (v_W & Core.Result.t_Result Prims.unit i1.f_Err)
+            (v_W & Core.Result.t_Result Prims.unit i1.f_Err))
+  }
+
+type t_Z_curve = { f_z_val:Hacspec_bip_340.t_Scalar }
+
+[@@ FStar.Tactics.Typeclasses.tcinstance]
+let impl: Concordium_contracts_common.Traits.t_Deserial t_Z_curve =
+  {
+    f_deserial_pre
+    =
+    (fun
+        (#v_R: Type0)
+        (#[FStar.Tactics.Typeclasses.tcresolve ()]
+          i1:
+          Concordium_contracts_common.Traits.t_Read v_R)
+        (source: v_R)
+        ->
+        true);
+    f_deserial_post
+    =
+    (fun
+        (#v_R: Type0)
+        (#[FStar.Tactics.Typeclasses.tcresolve ()]
+          i1:
+          Concordium_contracts_common.Traits.t_Read v_R)
+        (source: v_R)
+        (out1:
+          (v_R & Core.Result.t_Result t_Z_curve Concordium_contracts_common.Types.t_ParseError))
+        ->
+        true);
+    f_deserial
+    =
+    fun
+      (#v_R: Type0)
+      (#[FStar.Tactics.Typeclasses.tcresolve ()] i1: Concordium_contracts_common.Traits.t_Read v_R)
+      (source: v_R)
+      ->
+      let tmp0, out:(v_R &
+        Core.Result.t_Result (Alloc.Vec.t_Vec u8 Alloc.Alloc.t_Global)
+          Concordium_contracts_common.Types.t_ParseError) =
+        Concordium_contracts_common.Traits.f_get #v_R
+          #(Alloc.Vec.t_Vec u8 Alloc.Alloc.t_Global)
+          #FStar.Tactics.Typeclasses.solve
+          source
+      in
+      let source:v_R = tmp0 in
+      match out with
+      | Core.Result.Result_Ok (temp: Alloc.Vec.t_Vec u8 Alloc.Alloc.t_Global) ->
+        let hax_temp_output:Core.Result.t_Result t_Z_curve
+          Concordium_contracts_common.Types.t_ParseError =
+          Core.Result.Result_Ok
+          ({
+              f_z_val
+              =
+              Hacspec_bip_340.impl__Scalar__from_public_byte_seq_be #(Hacspec_lib.Seq.t_Seq u8)
+                (Hacspec_lib.Seq.impl_52__from_vec #u8 temp <: Hacspec_lib.Seq.t_Seq u8)
+            }
+            <:
+            t_Z_curve)
+          <:
+          Core.Result.t_Result t_Z_curve Concordium_contracts_common.Types.t_ParseError
+        in
+        source, hax_temp_output
+        <:
+        (v_R & Core.Result.t_Result t_Z_curve Concordium_contracts_common.Types.t_ParseError)
+      | Core.Result.Result_Err err ->
+        source,
+        (Core.Result.Result_Err err
+          <:
+          Core.Result.t_Result t_Z_curve Concordium_contracts_common.Types.t_ParseError)
+        <:
+        (v_R & Core.Result.t_Result t_Z_curve Concordium_contracts_common.Types.t_ParseError)
+  }
+
+[@@ FStar.Tactics.Typeclasses.tcinstance]
+let impl_1: Concordium_contracts_common.Traits.t_Serial t_Z_curve =
+  {
+    f_serial_pre
+    =
+    (fun
+        (#v_W: Type0)
+        (#[FStar.Tactics.Typeclasses.tcresolve ()]
+          i1:
+          Concordium_contracts_common.Traits.t_Write v_W)
+        (self: t_Z_curve)
+        (out: v_W)
+        ->
+        true);
+    f_serial_post
+    =
+    (fun
+        (#v_W: Type0)
+        (#[FStar.Tactics.Typeclasses.tcresolve ()]
+          i1:
+          Concordium_contracts_common.Traits.t_Write v_W)
+        (self: t_Z_curve)
+        (out: v_W)
+        (out2: (v_W & Core.Result.t_Result Prims.unit i1.f_Err))
+        ->
+        true);
+    f_serial
+    =
+    fun
+      (#v_W: Type0)
+      (#[FStar.Tactics.Typeclasses.tcresolve ()] i1: Concordium_contracts_common.Traits.t_Write v_W)
+      (self: t_Z_curve)
+      (out: v_W)
+      ->
+      let (v: Alloc.Vec.t_Vec u8 Alloc.Alloc.t_Global):Alloc.Vec.t_Vec u8 Alloc.Alloc.t_Global =
+        Alloc.Vec.impl__new #u8 ()
+      in
+      let v:Alloc.Vec.t_Vec u8 Alloc.Alloc.t_Global =
+        Core.Iter.Traits.Iterator.f_fold (Core.Iter.Traits.Collect.f_into_iter #(t_Slice u8)
+              #FStar.Tactics.Typeclasses.solve
+              (Hacspec_lib.Seq.impl_41__native_slice #u8
+                  (Hacspec_bip_340.impl__Scalar__to_public_byte_seq_be self.f_z_val
+                    <:
+                    Hacspec_lib.Seq.t_Seq u8)
+                <:
+                t_Slice u8)
+            <:
+            Core.Slice.Iter.t_Iter u8)
+          v
+          (fun v x ->
+              let v:Alloc.Vec.t_Vec u8 Alloc.Alloc.t_Global = v in
+              let x:u8 = x in
+              Alloc.Vec.impl_1__push #u8
+                #Alloc.Alloc.t_Global
+                v
+                (Core.Clone.f_clone #u8 #FStar.Tactics.Typeclasses.solve x <: u8)
+              <:
+              Alloc.Vec.t_Vec u8 Alloc.Alloc.t_Global)
+      in
+      let tmp0, out1:(v_W & Core.Result.t_Result Prims.unit i1.f_Err) =
+        Concordium_contracts_common.Traits.f_serial #(Alloc.Vec.t_Vec u8 Alloc.Alloc.t_Global)
+          #FStar.Tactics.Typeclasses.solve
+          #v_W
+          v
+          out
+      in
+      let out:v_W = tmp0 in
+      let hax_temp_output:Core.Result.t_Result Prims.unit i1.f_Err = out1 in
+      out, hax_temp_output <: (v_W & Core.Result.t_Result Prims.unit i1.f_Err)
+  }
+
+[@@ FStar.Tactics.Typeclasses.tcinstance]
+let impl_2: Hacspec_ovn.Ovn_traits.t_Field t_Z_curve =
+  {
+    _super_11581440318597584651 = FStar.Tactics.Typeclasses.solve;
+    _super_12632649257025169145 = FStar.Tactics.Typeclasses.solve;
+    _super_8099741844003281729 = FStar.Tactics.Typeclasses.solve;
+    _super_9442900250278684536 = FStar.Tactics.Typeclasses.solve;
+    _super_11581440318597584651 = FStar.Tactics.Typeclasses.solve;
+    _super_17605656595743636193 = FStar.Tactics.Typeclasses.solve;
+    f_q_pre = (fun (_: Prims.unit) -> true);
+    f_q_post = (fun (_: Prims.unit) (out: t_Z_curve) -> true);
+    f_q
+    =
+    (fun (_: Prims.unit) ->
+        {
+          f_z_val
+          =
+          Hacspec_bip_340.impl__Scalar__from_hex "0xFFFFFFFFFFFFFFFFFFFFFFFFFFFFFFFEBAAEDCE6AF48A03BBFD25E8CD0364141"
+
+        }
+        <:
+        t_Z_curve);
+    f_random_field_elem_pre = (fun (random: u32) -> true);
+    f_random_field_elem_post = (fun (random: u32) (out: t_Z_curve) -> true);
+    f_random_field_elem
+    =
+    (fun (random: u32) ->
+        { f_z_val = Hacspec_bip_340.impl__Scalar__from_literal (cast (random <: u32) <: u128) }
+        <:
+        t_Z_curve);
+    f_field_zero_pre = (fun (_: Prims.unit) -> true);
+    f_field_zero_post = (fun (_: Prims.unit) (out: t_Z_curve) -> true);
+    f_field_zero
+    =
+    (fun (_: Prims.unit) ->
+        { f_z_val = Hacspec_bip_340.impl__Scalar__from_literal (pub_u128 0) } <: t_Z_curve);
+    f_field_one_pre = (fun (_: Prims.unit) -> true);
+    f_field_one_post = (fun (_: Prims.unit) (out: t_Z_curve) -> true);
+    f_field_one
+    =
+    (fun (_: Prims.unit) ->
+        { f_z_val = Hacspec_bip_340.impl__Scalar__from_literal (pub_u128 1) } <: t_Z_curve);
+    f_add_pre = (fun (x: t_Z_curve) (y: t_Z_curve) -> true);
+    f_add_post = (fun (x: t_Z_curve) (y: t_Z_curve) (out: t_Z_curve) -> true);
+    f_add = (fun (x: t_Z_curve) (y: t_Z_curve) -> { f_z_val = x.f_z_val +! y.f_z_val } <: t_Z_curve);
+    f_opp_pre = (fun (x: t_Z_curve) -> true);
+    f_opp_post = (fun (x: t_Z_curve) (out: t_Z_curve) -> true);
+    f_opp
+    =
+    (fun (x: t_Z_curve) ->
+        {
+          f_z_val
+          =
+          (Hacspec_ovn.Ovn_traits.f_field_zero #t_Z_curve #FStar.Tactics.Typeclasses.solve ()
+            <:
+            t_Z_curve)
+            .f_z_val -!
+          x.f_z_val
+        }
+        <:
+        t_Z_curve);
+    f_mul_pre = (fun (x: t_Z_curve) (y: t_Z_curve) -> true);
+    f_mul_post = (fun (x: t_Z_curve) (y: t_Z_curve) (out: t_Z_curve) -> true);
+    f_mul = (fun (x: t_Z_curve) (y: t_Z_curve) -> { f_z_val = x.f_z_val *! y.f_z_val } <: t_Z_curve);
+    f_inv_pre = (fun (x: t_Z_curve) -> true);
+    f_inv_post = (fun (x: t_Z_curve) (out: t_Z_curve) -> true);
+    f_inv
+    =
+    fun (x: t_Z_curve) ->
+      Rust_primitives.Hax.Control_flow_monad.Mexception.run (let _:Prims.unit =
+            Hax_lib.v_assert false
+          in
+          let! hoist10:Rust_primitives.Hax.t_Never =
+            Core.Ops.Control_flow.ControlFlow_Break x
+            <:
+            Core.Ops.Control_flow.t_ControlFlow t_Z_curve Rust_primitives.Hax.t_Never
+          in
+          Core.Ops.Control_flow.ControlFlow_Continue (Rust_primitives.Hax.never_to_any hoist10)
+          <:
+          Core.Ops.Control_flow.t_ControlFlow t_Z_curve t_Z_curve)
+  }
+
+[@@ FStar.Tactics.Typeclasses.tcinstance]
+let impl_5: Hacspec_ovn.Ovn_traits.t_Group t_Group_curve =
+  {
+    _super_11581440318597584651 = FStar.Tactics.Typeclasses.solve;
+    _super_12632649257025169145 = FStar.Tactics.Typeclasses.solve;
+    _super_8099741844003281729 = FStar.Tactics.Typeclasses.solve;
+    _super_9442900250278684536 = FStar.Tactics.Typeclasses.solve;
+    _super_11581440318597584651 = FStar.Tactics.Typeclasses.solve;
+    _super_17605656595743636193 = FStar.Tactics.Typeclasses.solve;
+    f_Z = t_Z_curve;
+    f_Z_5568683927164688039 = FStar.Tactics.Typeclasses.solve;
+    f_g_pre = (fun (_: Prims.unit) -> true);
+    f_g_post = (fun (_: Prims.unit) (out: t_Group_curve) -> true);
+    f_g
+    =
+    (fun (_: Prims.unit) ->
+        let gx:Hacspec_bip_340.t_PBytes32 =
+          Hacspec_bip_340.PBytes32
+          (let list =
+              [
+                121uy; 190uy; 102uy; 126uy; 249uy; 220uy; 187uy; 172uy; 85uy; 160uy; 98uy; 149uy;
+                206uy; 135uy; 11uy; 7uy; 2uy; 155uy; 252uy; 219uy; 45uy; 206uy; 40uy; 217uy; 89uy;
+                242uy; 129uy; 91uy; 22uy; 248uy; 23uy; 152uy
+              ]
+            in
+            FStar.Pervasives.assert_norm (Prims.eq2 (List.Tot.length list) 32);
+            Rust_primitives.Hax.array_of_list 32 list)
+          <:
+          Hacspec_bip_340.t_PBytes32
+        in
+        let gy:Hacspec_bip_340.t_PBytes32 =
+          Hacspec_bip_340.PBytes32
+          (let list =
+              [
+                72uy; 58uy; 218uy; 119uy; 38uy; 163uy; 196uy; 101uy; 93uy; 164uy; 251uy; 252uy; 14uy;
+                17uy; 8uy; 168uy; 253uy; 23uy; 180uy; 72uy; 166uy; 133uy; 84uy; 25uy; 156uy; 71uy;
+                208uy; 143uy; 251uy; 16uy; 212uy; 184uy
+              ]
+            in
+            FStar.Pervasives.assert_norm (Prims.eq2 (List.Tot.length list) 32);
+            Rust_primitives.Hax.array_of_list 32 list)
+          <:
+          Hacspec_bip_340.t_PBytes32
+        in
+        {
+          f_g_val
+          =
+          Hacspec_bip_340.Point_Affine
+          (Hacspec_bip_340.impl__FieldElement__from_public_byte_seq_be #Hacspec_bip_340.t_PBytes32
+              gx,
+            Hacspec_bip_340.impl__FieldElement__from_public_byte_seq_be #Hacspec_bip_340.t_PBytes32
+              gy
+            <:
+            (Hacspec_bip_340.t_FieldElement & Hacspec_bip_340.t_FieldElement))
+          <:
+          Hacspec_bip_340.t_Point
+        }
+        <:
+        t_Group_curve);
+    f_pow_pre = (fun (g: t_Group_curve) (x: t_Z_curve) -> true);
+    f_pow_post = (fun (g: t_Group_curve) (x: t_Z_curve) (out: t_Group_curve) -> true);
+    f_pow
+    =
+    (fun (g: t_Group_curve) (x: t_Z_curve) ->
+        { f_g_val = Hacspec_bip_340.point_mul x.f_z_val g.f_g_val } <: t_Group_curve);
+    f_g_pow_pre = (fun (x: t_Z_curve) -> true);
+    f_g_pow_post = (fun (x: t_Z_curve) (out: t_Group_curve) -> true);
+    f_g_pow
+    =
+    (fun (x: t_Z_curve) -> { f_g_val = Hacspec_bip_340.point_mul_base x.f_z_val } <: t_Group_curve);
+    f_group_one_pre = (fun (_: Prims.unit) -> true);
+    f_group_one_post = (fun (_: Prims.unit) (out: t_Group_curve) -> true);
+    f_group_one
+    =
+    (fun (_: Prims.unit) ->
+        Hacspec_ovn.Ovn_traits.f_g_pow #t_Group_curve
+          #FStar.Tactics.Typeclasses.solve
+          (Hacspec_ovn.Ovn_traits.f_field_zero #t_Z_curve #FStar.Tactics.Typeclasses.solve ()
+            <:
+            t_Z_curve));
+    f_prod_pre = (fun (x: t_Group_curve) (y: t_Group_curve) -> true);
+    f_prod_post = (fun (x: t_Group_curve) (y: t_Group_curve) (out: t_Group_curve) -> true);
+    f_prod
+    =
+    (fun (x: t_Group_curve) (y: t_Group_curve) ->
+        { f_g_val = Hacspec_bip_340.point_add x.f_g_val y.f_g_val } <: t_Group_curve);
+    f_group_inv_pre = (fun (x: t_Group_curve) -> true);
+    f_group_inv_post = (fun (x: t_Group_curve) (out: t_Group_curve) -> true);
+    f_group_inv
+    =
+    (fun (x: t_Group_curve) ->
+        {
+          f_g_val
+          =
+          match x.f_g_val with
+          | Hacspec_bip_340.Point_Affine (a, b) ->
+            Hacspec_bip_340.Point_Affine
+            (a,
+              (Hacspec_bip_340.impl__FieldElement__from_literal (pub_u128 0)
+                <:
+                Hacspec_bip_340.t_FieldElement) -!
+              b
+              <:
+              (Hacspec_bip_340.t_FieldElement & Hacspec_bip_340.t_FieldElement))
+            <:
+            Hacspec_bip_340.t_Point
+          | Hacspec_bip_340.Point_AtInfinity  ->
+            Hacspec_bip_340.Point_AtInfinity <: Hacspec_bip_340.t_Point
+        }
+        <:
+        t_Group_curve);
+    f_hash_pre = (fun (x: Alloc.Vec.t_Vec t_Group_curve Alloc.Alloc.t_Global) -> true);
+    f_hash_post
+    =
+    (fun (x: Alloc.Vec.t_Vec t_Group_curve Alloc.Alloc.t_Global) (out: t_Z_curve) -> true);
+    f_hash
+    =
+    fun (x: Alloc.Vec.t_Vec t_Group_curve Alloc.Alloc.t_Global) ->
+      Hacspec_ovn.Ovn_traits.f_field_one #t_Z_curve #FStar.Tactics.Typeclasses.solve ()
+  }
