ovn/proofs/fstar/extraction/Hacspec_ovn.Ovn_z_89_.fst
@@ -1,0 +1,226 @@
+module Hacspec_ovn.Ovn_z_89_
+#set-options "--fuel 0 --ifuel 1 --z3rlimit 15"
+open Core
+open FStar.Mul
+
+let _ =
+  (* This module has implicit dependencies, here we make them explicit. *)
+  (* The implicit dependencies arise from typeclasses instances. *)
+  let open Concordium_contracts_common.Traits in
+  let open Hacspec_ovn.Ovn_traits in
+  ()
+
+type t_g_z_89_ = { f_g_val:u8 }
+
+type t_z_89_ = { f_z_val:u8 }
+
+[@@ FStar.Tactics.Typeclasses.tcinstance]
+let impl: Hacspec_ovn.Ovn_traits.t_Field t_z_89_ =
+  {
+    _super_11581440318597584651 = FStar.Tactics.Typeclasses.solve;
+    _super_12632649257025169145 = FStar.Tactics.Typeclasses.solve;
+    _super_8099741844003281729 = FStar.Tactics.Typeclasses.solve;
+    _super_9442900250278684536 = FStar.Tactics.Typeclasses.solve;
+    _super_11581440318597584651 = FStar.Tactics.Typeclasses.solve;
+    _super_17605656595743636193 = FStar.Tactics.Typeclasses.solve;
+    f_q_pre = (fun (_: Prims.unit) -> true);
+    f_q_post = (fun (_: Prims.unit) (out: t_z_89_) -> true);
+    f_q = (fun (_: Prims.unit) -> { f_z_val = 89uy } <: t_z_89_);
+    f_random_field_elem_pre = (fun (random: u32) -> true);
+    f_random_field_elem_post = (fun (random: u32) (out: t_z_89_) -> true);
+    f_random_field_elem
+    =
+    (fun (random: u32) ->
+        {
+          f_z_val
+          =
+          (cast (random <: u32) <: u8) %!
+          ((Hacspec_ovn.Ovn_traits.f_q #t_z_89_ #FStar.Tactics.Typeclasses.solve () <: t_z_89_)
+              .f_z_val -!
+            1uy
+            <:
+            u8)
+        }
+        <:
+        t_z_89_);
+    f_field_zero_pre = (fun (_: Prims.unit) -> true);
+    f_field_zero_post = (fun (_: Prims.unit) (out: t_z_89_) -> true);
+    f_field_zero = (fun (_: Prims.unit) -> { f_z_val = 0uy } <: t_z_89_);
+    f_field_one_pre = (fun (_: Prims.unit) -> true);
+    f_field_one_post = (fun (_: Prims.unit) (out: t_z_89_) -> true);
+    f_field_one = (fun (_: Prims.unit) -> { f_z_val = 1uy } <: t_z_89_);
+    f_add_pre = (fun (x: t_z_89_) (y: t_z_89_) -> true);
+    f_add_post = (fun (x: t_z_89_) (y: t_z_89_) (out: t_z_89_) -> true);
+    f_add
+    =
+    (fun (x: t_z_89_) (y: t_z_89_) ->
+        let q___:u8 =
+          (Hacspec_ovn.Ovn_traits.f_q #t_z_89_ #FStar.Tactics.Typeclasses.solve () <: t_z_89_)
+            .f_z_val -!
+          1uy
+        in
+        let x___:u8 = x.f_z_val %! q___ in
+        let y___:u8 = y.f_z_val %! q___ in
+        { f_z_val = (x___ +! y___ <: u8) %! q___ } <: t_z_89_);
+    f_opp_pre = (fun (x: t_z_89_) -> true);
+    f_opp_post = (fun (x: t_z_89_) (out: t_z_89_) -> true);
+    f_opp
+    =
+    (fun (x: t_z_89_) ->
+        let q___:u8 =
+          (Hacspec_ovn.Ovn_traits.f_q #t_z_89_ #FStar.Tactics.Typeclasses.solve () <: t_z_89_)
+            .f_z_val -!
+          1uy
+        in
+        let x___:u8 = x.f_z_val %! q___ in
+        { f_z_val = q___ -! x___ } <: t_z_89_);
+    f_mul_pre = (fun (x: t_z_89_) (y: t_z_89_) -> true);
+    f_mul_post = (fun (x: t_z_89_) (y: t_z_89_) (out: t_z_89_) -> true);
+    f_mul
+    =
+    (fun (x: t_z_89_) (y: t_z_89_) ->
+        let q___:u8 =
+          (Hacspec_ovn.Ovn_traits.f_q #t_z_89_ #FStar.Tactics.Typeclasses.solve () <: t_z_89_)
+            .f_z_val -!
+          1uy
+        in
+        let (x___: u16):u16 = cast (x.f_z_val %! q___ <: u8) <: u16 in
+        let (y___: u16):u16 = cast (y.f_z_val %! q___ <: u8) <: u16 in
+        { f_z_val = cast ((x___ *! y___ <: u16) %! (cast (q___ <: u8) <: u16) <: u16) <: u8 }
+        <:
+        t_z_89_);
+    f_inv_pre = (fun (x: t_z_89_) -> true);
+    f_inv_post = (fun (x: t_z_89_) (out: t_z_89_) -> true);
+    f_inv
+    =
+    fun (x: t_z_89_) ->
+      Rust_primitives.Hax.Control_flow_monad.Mexception.run (let _:Prims.unit =
+            Hax_lib.v_assert false
+          in
+          let! hoist11:Rust_primitives.Hax.t_Never =
+            Core.Ops.Control_flow.ControlFlow_Break x
+            <:
+            Core.Ops.Control_flow.t_ControlFlow t_z_89_ Rust_primitives.Hax.t_Never
+          in
+          Core.Ops.Control_flow.ControlFlow_Continue (Rust_primitives.Hax.never_to_any hoist11)
+          <:
+          Core.Ops.Control_flow.t_ControlFlow t_z_89_ t_z_89_)
+  }
+
+[@@ FStar.Tactics.Typeclasses.tcinstance]
+let impl_1: Hacspec_ovn.Ovn_traits.t_Group t_g_z_89_ =
+  {
+    _super_11581440318597584651 = FStar.Tactics.Typeclasses.solve;
+    _super_12632649257025169145 = FStar.Tactics.Typeclasses.solve;
+    _super_8099741844003281729 = FStar.Tactics.Typeclasses.solve;
+    _super_9442900250278684536 = FStar.Tactics.Typeclasses.solve;
+    _super_11581440318597584651 = FStar.Tactics.Typeclasses.solve;
+    _super_17605656595743636193 = FStar.Tactics.Typeclasses.solve;
+    f_Z = t_z_89_;
+    f_Z_5568683927164688039 = FStar.Tactics.Typeclasses.solve;
+    f_g_pre = (fun (_: Prims.unit) -> true);
+    f_g_post = (fun (_: Prims.unit) (out: t_g_z_89_) -> true);
+    f_g = (fun (_: Prims.unit) -> { f_g_val = 3uy } <: t_g_z_89_);
+    f_hash_pre = (fun (x: Alloc.Vec.t_Vec t_g_z_89_ Alloc.Alloc.t_Global) -> true);
+    f_hash_post = (fun (x: Alloc.Vec.t_Vec t_g_z_89_ Alloc.Alloc.t_Global) (out: t_z_89_) -> true);
+    f_hash
+    =
+    (fun (x: Alloc.Vec.t_Vec t_g_z_89_ Alloc.Alloc.t_Global) ->
+        let res:t_z_89_ =
+          Hacspec_ovn.Ovn_traits.f_field_one #t_z_89_ #FStar.Tactics.Typeclasses.solve ()
+        in
+        let res:t_z_89_ =
+          Core.Iter.Traits.Iterator.f_fold (Core.Iter.Traits.Collect.f_into_iter #(Alloc.Vec.t_Vec
+                    t_g_z_89_ Alloc.Alloc.t_Global)
+                #FStar.Tactics.Typeclasses.solve
+                x
+              <:
+              Alloc.Vec.Into_iter.t_IntoIter t_g_z_89_ Alloc.Alloc.t_Global)
+            res
+            (fun res y ->
+                let res:t_z_89_ = res in
+                let y:t_g_z_89_ = y in
+                Hacspec_ovn.Ovn_traits.f_mul #t_z_89_
+                  #FStar.Tactics.Typeclasses.solve
+                  ({ f_z_val = y.f_g_val } <: t_z_89_)
+                  res
+                <:
+                t_z_89_)
+        in
+        res);
+    f_g_pow_pre = (fun (x: t_z_89_) -> true);
+    f_g_pow_post = (fun (x: t_z_89_) (out: t_g_z_89_) -> true);
+    f_g_pow
+    =
+    (fun (x: t_z_89_) ->
+        Hacspec_ovn.Ovn_traits.f_pow #t_g_z_89_
+          #FStar.Tactics.Typeclasses.solve
+          (Hacspec_ovn.Ovn_traits.f_g #t_g_z_89_ #FStar.Tactics.Typeclasses.solve () <: t_g_z_89_)
+          x);
+    f_pow_pre = (fun (g: t_g_z_89_) (x: t_z_89_) -> true);
+    f_pow_post = (fun (g: t_g_z_89_) (x: t_z_89_) (out: t_g_z_89_) -> true);
+    f_pow
+    =
+    (fun (g: t_g_z_89_) (x: t_z_89_) ->
+        let result:t_g_z_89_ =
+          Hacspec_ovn.Ovn_traits.f_group_one #t_g_z_89_ #FStar.Tactics.Typeclasses.solve ()
+        in
+        let result:t_g_z_89_ =
+          Rust_primitives.Hax.Folds.fold_range 0uy
+            (x.f_z_val %!
+              ((Hacspec_ovn.Ovn_traits.f_q #t_z_89_ #FStar.Tactics.Typeclasses.solve () <: t_z_89_)
+                  .f_z_val -!
+                1uy
+                <:
+                u8)
+              <:
+              u8)
+            (fun result temp_1_ ->
+                let result:t_g_z_89_ = result in
+                let _:u8 = temp_1_ in
+                true)
+            result
+            (fun result temp_1_ ->
+                let result:t_g_z_89_ = result in
+                let _:u8 = temp_1_ in
+                Hacspec_ovn.Ovn_traits.f_prod #t_g_z_89_ #FStar.Tactics.Typeclasses.solve result g
+                <:
+                t_g_z_89_)
+        in
+        result);
+    f_group_one_pre = (fun (_: Prims.unit) -> true);
+    f_group_one_post = (fun (_: Prims.unit) (out: t_g_z_89_) -> true);
+    f_group_one = (fun (_: Prims.unit) -> { f_g_val = 1uy } <: t_g_z_89_);
+    f_prod_pre = (fun (x: t_g_z_89_) (y: t_g_z_89_) -> true);
+    f_prod_post = (fun (x: t_g_z_89_) (y: t_g_z_89_) (out: t_g_z_89_) -> true);
+    f_prod
+    =
+    (fun (x: t_g_z_89_) (y: t_g_z_89_) ->
+        let q___:u8 =
+          (Hacspec_ovn.Ovn_traits.f_q #t_z_89_ #FStar.Tactics.Typeclasses.solve ()).f_z_val
+        in
+        let x___:u16 = cast (x.f_g_val %! q___ <: u8) <: u16 in
+        let y___:u16 = cast (y.f_g_val %! q___ <: u8) <: u16 in
+        { f_g_val = cast ((x___ *! y___ <: u16) %! (cast (q___ <: u8) <: u16) <: u16) <: u8 }
+        <:
+        t_g_z_89_);
+    f_group_inv_pre = (fun (x: t_g_z_89_) -> true);
+    f_group_inv_post = (fun (x: t_g_z_89_) (out: t_g_z_89_) -> true);
+    f_group_inv
+    =
+    fun (x: t_g_z_89_) ->
+      Rust_primitives.Hax.Control_flow_monad.Mexception.run (let _:Prims.unit =
+            Rust_primitives.Hax.failure "(FunctionalizeLoops) something is not implemented yet.\nLoop without mutation?"
+              "{\n        for j in (core::iter::traits::collect::f_into_iter(core::ops::range::Range {\n            f_start: 0,\n            f_end: 89,\n        })) {\n            {\n                let g_value: hacspec_ovn::ovn_z_89_::t_g_z_89_ = {\n                    hacspec_ovn::ovn_z_89_::C_g_z_89_ {\n                        f_g_val: j,\n                    }\n                };\n                (if core::cmp::f_eq(\n                    hacspec_ovn::ovn_traits::f_prod(x, g_value),\n                    hacspec_ovn::ovn_traits::f_group_one(Tuple0),\n                ) {\n                    {\n                        #[note(\n                            \"rhs.typ=core::ops::control_flow::t_ControlFlow<hacspec_ovn::ovn_z_89_::t_g_z_89_, rust_primitives::hax::t_Never>\"\n                        )]\n                        #[monadic_let(MException<hacspec_ovn::ovn_z_89_::t_g_z_89_>)]\n                        let hoist15: rust_primitives::hax::t_Never = {\n                            core::ops::control_flow::ControlFlow_Break(g_value)\n                        };\n                        core::ops::control_flow::ControlFlow_Continue(\n                            rust_primitives::hax::never_to_any(hoist15),\n                        )\n                    }\n                } else {\n                    core::ops::control_flow::ControlFlow_Continue(Tuple0)\n                })\n            }\n        }\n    }"
+
+          in
+          let _:Prims.unit = Hax_lib.v_assert false in
+          let! hoist16:Rust_primitives.Hax.t_Never =
+            Core.Ops.Control_flow.ControlFlow_Break x
+            <:
+            Core.Ops.Control_flow.t_ControlFlow t_g_z_89_ Rust_primitives.Hax.t_Never
+          in
+          Core.Ops.Control_flow.ControlFlow_Continue (Rust_primitives.Hax.never_to_any hoist16)
+          <:
+          Core.Ops.Control_flow.t_ControlFlow t_g_z_89_ t_g_z_89_)
+  }
