ovn/proofs/ssprove/extraction/Hacspec_ovn_Ovn_group2.v
@@ -27,39 +27,42 @@ Obligation Tactic := (* try timeout 8 *) solve_ssprove_obligations.
 Require Import Crate_Ovn_traits.
 Export Crate_Ovn_traits.
 
-Equations sub {v_Z : _} `{ t_Sized v_Z} `{ t_Field v_Z} (x : both v_Z) (y : both v_Z) : both v_Z :=
-  sub x y  :=
-    x .+ (f_neg y) : both v_Z.
-Fail Next Obligation.
+Require Import PhantomData.
+Export PhantomData.
 
-Equations compute_group_element_for_vote {v_G : _} `{ t_Sized v_G} `{ t_Group v_G} (xi : both f_Z) (vote : both 'bool) (g_pow_yi : both v_G) : both v_G :=
-  compute_group_element_for_vote xi vote g_pow_yi  :=
+Equations impl__compute_group_element_for_vote {v_G : _} `{ t_Sized v_G} `{ t_Group v_G} (xi : both f_Z) (vote : both 'bool) (g_pow_yi : both v_G) : both v_G :=
+  impl__compute_group_element_for_vote xi vote g_pow_yi  :=
     (f_pow g_pow_yi xi) .* (f_g_pow (ifb vote
     then f_field_one
     else f_field_zero)) : both v_G.
 Fail Next Obligation.
 
-Equations div {v_G : _} `{ t_Sized v_G} `{ t_Group v_G} (x : both v_G) (y : both v_G) : both v_G :=
-  div x y  :=
+Equations impl__div {v_G : _} `{ t_Sized v_G} `{ t_Group v_G} (x : both v_G) (y : both v_G) : both v_G :=
+  impl__div x y  :=
     x .* (f_group_inv y) : both v_G.
 Fail Next Obligation.
 
-Equations compute_g_pow_yi {v_G : _} {n : both uint_size} `{ t_Sized v_G} `{ t_Group v_G} (i : both uint_size) (xis : both (nseq v_G (is_pure (n)))) : both v_G :=
-  compute_g_pow_yi i xis  :=
+Equations impl__compute_g_pow_yi {v_G : _} {n : both uint_size} `{ t_Sized v_G} `{ t_Group v_G} (i : both uint_size) (xis : both (nseq v_G (is_pure (n)))) : both v_G :=
+  impl__compute_g_pow_yi i xis  :=
     letb prod1 := f_product (f_map (impl__iter (xis.a[(Build_t_Range (f_start := ret_both (0 : uint_size)) (f_end := i))])) (fun x =>
       f_clone x)) in
     letb prod2 := f_product (f_map (impl__iter (xis.a[(Build_t_Range (f_start := i .+ (ret_both (1 : uint_size))) (f_end := n))])) (fun x =>
       f_clone x)) in
-    div prod1 prod2 : both v_G.
+    impl__div prod1 prod2 : both v_G.
 Fail Next Obligation.
 
-Equations check_commitment {v_G : _} `{ t_Sized v_G} `{ t_Group v_G} (g_pow_xi_yi_vi : both v_G) (commitment : both f_Z) : both 'bool :=
-  check_commitment g_pow_xi_yi_vi commitment  :=
+Equations impl__sub {v_G : _} `{ t_Sized v_G} `{ t_Group v_G} (x : both f_Z) (y : both f_Z) : both f_Z :=
+  impl__sub x y  :=
+    x .+ (f_neg y) : both f_Z.
+Fail Next Obligation.
+
+Equations impl__check_commitment {v_G : _} `{ t_Sized v_G} `{ t_Group v_G} (g_pow_xi_yi_vi : both v_G) (commitment : both f_Z) : both 'bool :=
+  impl__check_commitment g_pow_xi_yi_vi commitment  :=
     (f_hash (impl__into_vec (unsize (box_new (array_from_list [g_pow_xi_yi_vi]))))) =.? commitment : both 'bool.
 Fail Next Obligation.
 
-Equations commit_to {v_G : _} `{ t_Sized v_G} `{ t_Group v_G} (g_pow_xi_yi_vi : both v_G) : both f_Z :=
-  commit_to g_pow_xi_yi_vi  :=
+Equations impl__commit_to {v_G : _} `{ t_Sized v_G} `{ t_Group v_G} (g_pow_xi_yi_vi : both v_G) : both f_Z :=
+  impl__commit_to g_pow_xi_yi_vi  :=
     f_hash (impl__into_vec (unsize (box_new (array_from_list [g_pow_xi_yi_vi])))) : both f_Z.
 Fail Next Obligation.
 
@@ -111,6 +114,20 @@ Notation "'Build_t_CastVoteParam' '[' x ']' '(' 'f_cvp_zkp_random_w' ':=' y ')'"
 Notation "'Build_t_CastVoteParam' '[' x ']' '(' 'f_cvp_zkp_random_r' ':=' y ')'" := (Build_t_CastVoteParam (f_cvp_i := f_cvp_i x) (f_cvp_xi := f_cvp_xi x) (f_cvp_zkp_random_w := f_cvp_zkp_random_w x) (f_cvp_zkp_random_r := y) (f_cvp_zkp_random_d := f_cvp_zkp_random_d x) (f_cvp_vote := f_cvp_vote x)).
 Notation "'Build_t_CastVoteParam' '[' x ']' '(' 'f_cvp_zkp_random_d' ':=' y ')'" := (Build_t_CastVoteParam (f_cvp_i := f_cvp_i x) (f_cvp_xi := f_cvp_xi x) (f_cvp_zkp_random_w := f_cvp_zkp_random_w x) (f_cvp_zkp_random_r := f_cvp_zkp_random_r x) (f_cvp_zkp_random_d := y) (f_cvp_vote := f_cvp_vote x)).
 Notation "'Build_t_CastVoteParam' '[' x ']' '(' 'f_cvp_vote' ':=' y ')'" := (Build_t_CastVoteParam (f_cvp_i := f_cvp_i x) (f_cvp_xi := f_cvp_xi x) (f_cvp_zkp_random_w := f_cvp_zkp_random_w x) (f_cvp_zkp_random_r := f_cvp_zkp_random_r x) (f_cvp_zkp_random_d := f_cvp_zkp_random_d x) (f_cvp_vote := y)).
+
+Definition t_OVN {v_G : _} `{ t_Sized v_G} `{ t_Group v_G} : choice_type :=
+  (t_PhantomData v_G).
+Equations f_pd {v_G : _} `{ t_Sized v_G} `{ t_Group v_G} (s : both t_OVN) : both (t_PhantomData v_G) :=
+  f_pd s  :=
+    bind_both s (fun x =>
+      ret_both (x : (t_PhantomData v_G))) : both (t_PhantomData v_G).
+Fail Next Obligation.
+Equations Build_t_OVN {v_G : _} `{ t_Sized v_G} `{ t_Group v_G} {f_pd : both (t_PhantomData v_G)} : both (t_OVN) :=
+  Build_t_OVN  :=
+    bind_both f_pd (fun f_pd =>
+      ret_both ((f_pd) : (t_OVN))) : both (t_OVN).
+Fail Next Obligation.
+Notation "'Build_t_OVN' '[' x ']' '(' 'f_pd' ':=' y ')'" := (Build_t_OVN (f_pd := y)).
 
 Definition t_OrZKPCommit {v_G : _} `{ t_Sized v_G} `{ t_Group v_G} : choice_type :=
   (v_G × v_G × v_G × v_G × v_G × v_G × f_Z × f_Z × f_Z × f_Z × f_Z).
@@ -196,6 +213,57 @@ Notation "'Build_t_OrZKPCommit' '[' x ']' '(' 'f_or_zkp_d2' ':=' y ')'" := (Buil
 Notation "'Build_t_OrZKPCommit' '[' x ']' '(' 'f_or_zkp_r1' ':=' y ')'" := (Build_t_OrZKPCommit (f_or_zkp_x := f_or_zkp_x x) (f_or_zkp_y := f_or_zkp_y x) (f_or_zkp_a1 := f_or_zkp_a1 x) (f_or_zkp_b1 := f_or_zkp_b1 x) (f_or_zkp_a2 := f_or_zkp_a2 x) (f_or_zkp_b2 := f_or_zkp_b2 x) (f_or_zkp_c := f_or_zkp_c x) (f_or_zkp_d1 := f_or_zkp_d1 x) (f_or_zkp_d2 := f_or_zkp_d2 x) (f_or_zkp_r1 := y) (f_or_zkp_r2 := f_or_zkp_r2 x)).
 Notation "'Build_t_OrZKPCommit' '[' x ']' '(' 'f_or_zkp_r2' ':=' y ')'" := (Build_t_OrZKPCommit (f_or_zkp_x := f_or_zkp_x x) (f_or_zkp_y := f_or_zkp_y x) (f_or_zkp_a1 := f_or_zkp_a1 x) (f_or_zkp_b1 := f_or_zkp_b1 x) (f_or_zkp_a2 := f_or_zkp_a2 x) (f_or_zkp_b2 := f_or_zkp_b2 x) (f_or_zkp_c := f_or_zkp_c x) (f_or_zkp_d1 := f_or_zkp_d1 x) (f_or_zkp_d2 := f_or_zkp_d2 x) (f_or_zkp_r1 := f_or_zkp_r1 x) (f_or_zkp_r2 := y)).
 
+Equations impl__zkp_one_out_of_two {v_G : _} `{ t_Sized v_G} `{ t_Group v_G} (random_w : both f_Z) (random_r : both f_Z) (random_d : both f_Z) (h : both v_G) (xi : both f_Z) (vi : both 'bool) : both (t_OrZKPCommit v_G) :=
+  impl__zkp_one_out_of_two random_w random_r random_d h xi vi  :=
+    letb w := random_w in
+    ifb vi
+    then letb r1 := random_r in
+    letb d1 := random_d in
+    letb x := f_g_pow xi in
+    letb y := (f_pow h xi) .* f_g in
+    letb a1 := (f_g_pow r1) .* (f_pow x d1) in
+    letb b1 := (f_pow h r1) .* (f_pow y d1) in
+    letb a2 := f_g_pow w in
+    letb b2 := f_pow h w in
+    letb c := f_hash (impl__into_vec (unsize (box_new (array_from_list [x;
+      y;
+      a1;
+      b1;
+      a2;
+      b2])))) in
+    letb d2 := impl__sub c d1 in
+    letb r2 := impl__sub w (xi .* d2) in
+    Build_t_OrZKPCommit (f_or_zkp_x := x) (f_or_zkp_y := y) (f_or_zkp_a1 := a1) (f_or_zkp_b1 := b1) (f_or_zkp_a2 := a2) (f_or_zkp_b2 := b2) (f_or_zkp_c := c) (f_or_zkp_d1 := d1) (f_or_zkp_d2 := d2) (f_or_zkp_r1 := r1) (f_or_zkp_r2 := r2)
+    else letb r2 := random_r in
+    letb d2 := random_d in
+    letb x := f_g_pow xi in
+    letb y := f_pow h xi in
+    letb a1 := f_g_pow w in
+    letb b1 := f_pow h w in
+    letb a2 := (f_g_pow r2) .* (f_pow x d2) in
+    letb b2 := (f_pow h r2) .* (f_pow (impl__div y f_g) d2) in
+    letb c := f_hash (impl__into_vec (unsize (box_new (array_from_list [x;
+      y;
+      a1;
+      b1;
+      a2;
+      b2])))) in
+    letb d1 := impl__sub c d2 in
+    letb r1 := impl__sub w (xi .* d1) in
+    Build_t_OrZKPCommit (f_or_zkp_x := x) (f_or_zkp_y := y) (f_or_zkp_a1 := a1) (f_or_zkp_b1 := b1) (f_or_zkp_a2 := a2) (f_or_zkp_b2 := b2) (f_or_zkp_c := c) (f_or_zkp_d1 := d1) (f_or_zkp_d2 := d2) (f_or_zkp_r1 := r1) (f_or_zkp_r2 := r2) : both (t_OrZKPCommit v_G).
+Fail Next Obligation.
+
+Equations impl__zkp_one_out_of_two_validate {v_G : _} `{ t_Sized v_G} `{ t_Group v_G} (h : both v_G) (zkp : both (t_OrZKPCommit v_G)) : both 'bool :=
+  impl__zkp_one_out_of_two_validate h zkp  :=
+    letb c := f_hash (impl__into_vec (unsize (box_new (array_from_list [f_or_zkp_x zkp;
+      f_or_zkp_y zkp;
+      f_or_zkp_a1 zkp;
+      f_or_zkp_b1 zkp;
+      f_or_zkp_a2 zkp;
+      f_or_zkp_b2 zkp])))) in
+    andb (andb (andb (andb (c =.? ((f_or_zkp_d1 zkp) .+ (f_or_zkp_d2 zkp))) ((f_or_zkp_a1 zkp) =.? ((f_g_pow (f_or_zkp_r1 zkp)) .* (f_pow (f_or_zkp_x zkp) (f_or_zkp_d1 zkp))))) ((f_or_zkp_b1 zkp) =.? ((f_pow h (f_or_zkp_r1 zkp)) .* (f_pow (f_or_zkp_y zkp) (f_or_zkp_d1 zkp))))) ((f_or_zkp_a2 zkp) =.? ((f_g_pow (f_or_zkp_r2 zkp)) .* (f_pow (f_or_zkp_x zkp) (f_or_zkp_d2 zkp))))) ((f_or_zkp_b2 zkp) =.? ((f_pow h (f_or_zkp_r2 zkp)) .* (f_pow (impl__div (f_or_zkp_y zkp) f_g) (f_or_zkp_d2 zkp)))) : both 'bool.
+Fail Next Obligation.
+
 Definition t_RegisterParam {v_Z : _} `{ t_Sized v_Z} `{ t_Field v_Z} : choice_type :=
   (int32 × v_Z × v_Z).
 Equations f_rp_i {v_Z : _} `{ t_Sized v_Z} `{ t_Field v_Z} (s : both t_RegisterParam) : both int32 :=
@@ -252,81 +320,30 @@ Notation "'Build_t_SchnorrZKPCommit' '[' x ']' '(' 'f_schnorr_zkp_u' ':=' y ')'"
 Notation "'Build_t_SchnorrZKPCommit' '[' x ']' '(' 'f_schnorr_zkp_c' ':=' y ')'" := (Build_t_SchnorrZKPCommit (f_schnorr_zkp_u := f_schnorr_zkp_u x) (f_schnorr_zkp_c := y) (f_schnorr_zkp_z := f_schnorr_zkp_z x)).
 Notation "'Build_t_SchnorrZKPCommit' '[' x ']' '(' 'f_schnorr_zkp_z' ':=' y ')'" := (Build_t_SchnorrZKPCommit (f_schnorr_zkp_u := f_schnorr_zkp_u x) (f_schnorr_zkp_c := f_schnorr_zkp_c x) (f_schnorr_zkp_z := y)).
 
-Definition t_TallyParameter : choice_type :=
-  'unit.
-Equations Build_t_TallyParameter : both (t_TallyParameter) :=
-  Build_t_TallyParameter  :=
-    ret_both (tt (* Empty tuple *) : (t_TallyParameter)) : both (t_TallyParameter).
-Fail Next Obligation.
-
-Equations schnorr_zkp {v_G : _} `{ t_Sized v_G} `{ t_Group v_G} (random : both f_Z) (h : both v_G) (x : both f_Z) : both (t_SchnorrZKPCommit v_G) :=
-  schnorr_zkp random h x  :=
+Equations impl__schnorr_zkp {v_G : _} `{ t_Sized v_G} `{ t_Group v_G} (random : both f_Z) (h : both v_G) (x : both f_Z) : both (t_SchnorrZKPCommit v_G) :=
+  impl__schnorr_zkp random h x  :=
     run (letb r := random in
     letb u := f_g_pow r in
     letb c := f_hash (impl__into_vec (unsize (box_new (array_from_list [f_g;
       h;
       u])))) in
     letb z := r .+ (c .* x) in
-    letm[choice_typeMonad.result_bind_code (t_SchnorrZKPCommit v_G)] hoist1 := ControlFlow_Break (Build_t_SchnorrZKPCommit (f_schnorr_zkp_u := u) (f_schnorr_zkp_c := c) (f_schnorr_zkp_z := z)) in
-    ControlFlow_Continue (never_to_any hoist1)) : both (t_SchnorrZKPCommit v_G).
+    letm[choice_typeMonad.result_bind_code (t_SchnorrZKPCommit v_G)] hoist2 := ControlFlow_Break (Build_t_SchnorrZKPCommit (f_schnorr_zkp_u := u) (f_schnorr_zkp_c := c) (f_schnorr_zkp_z := z)) in
+    ControlFlow_Continue (never_to_any hoist2)) : both (t_SchnorrZKPCommit v_G).
 Fail Next Obligation.
 
-Equations schnorr_zkp_validate {v_G : _} `{ t_Sized v_G} `{ t_Group v_G} (h : both v_G) (pi : both (t_SchnorrZKPCommit v_G)) : both 'bool :=
-  schnorr_zkp_validate h pi  :=
+Equations impl__schnorr_zkp_validate {v_G : _} `{ t_Sized v_G} `{ t_Group v_G} (h : both v_G) (pi : both (t_SchnorrZKPCommit v_G)) : both 'bool :=
+  impl__schnorr_zkp_validate h pi  :=
     andb ((f_schnorr_zkp_c pi) =.? (f_hash (impl__into_vec (unsize (box_new (array_from_list [f_g;
       h;
       f_schnorr_zkp_u pi])))))) ((f_g_pow (f_schnorr_zkp_z pi)) =.? ((f_schnorr_zkp_u pi) .* (f_pow h (f_schnorr_zkp_c pi)))) : both 'bool.
 Fail Next Obligation.
 
-Equations zkp_one_out_of_two {v_G : _} `{ t_Sized v_G} `{ t_Group v_G} (random_w : both f_Z) (random_r : both f_Z) (random_d : both f_Z) (h : both v_G) (xi : both f_Z) (vi : both 'bool) : both (t_OrZKPCommit v_G) :=
-  zkp_one_out_of_two random_w random_r random_d h xi vi  :=
-    letb w := random_w in
-    ifb vi
-    then letb r1 := random_r in
-    letb d1 := random_d in
-    letb x := f_g_pow xi in
-    letb y := (f_pow h xi) .* f_g in
-    letb a1 := (f_g_pow r1) .* (f_pow x d1) in
-    letb b1 := (f_pow h r1) .* (f_pow y d1) in
-    letb a2 := f_g_pow w in
-    letb b2 := f_pow h w in
-    letb c := f_hash (impl__into_vec (unsize (box_new (array_from_list [x;
-      y;
-      a1;
-      b1;
-      a2;
-      b2])))) in
-    letb d2 := sub c d1 in
-    letb r2 := sub w (xi .* d2) in
-    Build_t_OrZKPCommit (f_or_zkp_x := x) (f_or_zkp_y := y) (f_or_zkp_a1 := a1) (f_or_zkp_b1 := b1) (f_or_zkp_a2 := a2) (f_or_zkp_b2 := b2) (f_or_zkp_c := c) (f_or_zkp_d1 := d1) (f_or_zkp_d2 := d2) (f_or_zkp_r1 := r1) (f_or_zkp_r2 := r2)
-    else letb r2 := random_r in
-    letb d2 := random_d in
-    letb x := f_g_pow xi in
-    letb y := f_pow h xi in
-    letb a1 := f_g_pow w in
-    letb b1 := f_pow h w in
-    letb a2 := (f_g_pow r2) .* (f_pow x d2) in
-    letb b2 := (f_pow h r2) .* (f_pow (div y f_g) d2) in
-    letb c := f_hash (impl__into_vec (unsize (box_new (array_from_list [x;
-      y;
-      a1;
-      b1;
-      a2;
-      b2])))) in
-    letb d1 := sub c d2 in
-    letb r1 := sub w (xi .* d1) in
-    Build_t_OrZKPCommit (f_or_zkp_x := x) (f_or_zkp_y := y) (f_or_zkp_a1 := a1) (f_or_zkp_b1 := b1) (f_or_zkp_a2 := a2) (f_or_zkp_b2 := b2) (f_or_zkp_c := c) (f_or_zkp_d1 := d1) (f_or_zkp_d2 := d2) (f_or_zkp_r1 := r1) (f_or_zkp_r2 := r2) : both (t_OrZKPCommit v_G).
-Fail Next Obligation.
-
-Equations zkp_one_out_of_two_validate {v_G : _} `{ t_Sized v_G} `{ t_Group v_G} (h : both v_G) (zkp : both (t_OrZKPCommit v_G)) : both 'bool :=
-  zkp_one_out_of_two_validate h zkp  :=
-    letb c := f_hash (impl__into_vec (unsize (box_new (array_from_list [f_or_zkp_x zkp;
-      f_or_zkp_y zkp;
-      f_or_zkp_a1 zkp;
-      f_or_zkp_b1 zkp;
-      f_or_zkp_a2 zkp;
-      f_or_zkp_b2 zkp])))) in
-    andb (andb (andb (andb (c =.? ((f_or_zkp_d1 zkp) .+ (f_or_zkp_d2 zkp))) ((f_or_zkp_a1 zkp) =.? ((f_g_pow (f_or_zkp_r1 zkp)) .* (f_pow (f_or_zkp_x zkp) (f_or_zkp_d1 zkp))))) ((f_or_zkp_b1 zkp) =.? ((f_pow h (f_or_zkp_r1 zkp)) .* (f_pow (f_or_zkp_y zkp) (f_or_zkp_d1 zkp))))) ((f_or_zkp_a2 zkp) =.? ((f_g_pow (f_or_zkp_r2 zkp)) .* (f_pow (f_or_zkp_x zkp) (f_or_zkp_d2 zkp))))) ((f_or_zkp_b2 zkp) =.? ((f_pow h (f_or_zkp_r2 zkp)) .* (f_pow (div (f_or_zkp_y zkp) f_g) (f_or_zkp_d2 zkp)))) : both 'bool.
+Definition t_TallyParameter : choice_type :=
+  'unit.
+Equations Build_t_TallyParameter : both (t_TallyParameter) :=
+  Build_t_TallyParameter  :=
+    ret_both (tt (* Empty tuple *) : (t_TallyParameter)) : both (t_TallyParameter).
 Fail Next Obligation.
 
 Definition t_OvnContractState {v_G : _} {n : both uint_size} `{ t_Sized v_G} `{ t_Group v_G} : choice_type :=
@@ -385,48 +402,48 @@ Notation "'Build_t_OvnContractState' '[' x ']' '(' 'f_zkp_vis' ':=' y ')'" := (B
 Notation "'Build_t_OvnContractState' '[' x ']' '(' 'f_tally' ':=' y ')'" := (Build_t_OvnContractState (f_g_pow_xis := f_g_pow_xis x) (f_zkp_xis := f_zkp_xis x) (f_commit_vis := f_commit_vis x) (f_g_pow_xi_yi_vis := f_g_pow_xi_yi_vis x) (f_zkp_vis := f_zkp_vis x) (f_tally := y) (f_round1 := f_round1 x)).
 Notation "'Build_t_OvnContractState' '[' x ']' '(' 'f_round1' ':=' y ')'" := (Build_t_OvnContractState (f_g_pow_xis := f_g_pow_xis x) (f_zkp_xis := f_zkp_xis x) (f_commit_vis := f_commit_vis x) (f_g_pow_xi_yi_vis := f_g_pow_xi_yi_vis x) (f_zkp_vis := f_zkp_vis x) (f_tally := f_tally x) (f_round1 := y)).
 
-Equations cast_vote {v_G : _} {n : both uint_size} {v_A : _} {impl_574521470_ : _} `{ t_Sized v_G} `{ t_Sized v_A} `{ t_Sized impl_574521470_} `{ t_Group v_G} `{ t_HasActions v_A} `{ t_HasReceiveContext impl_574521470_ 'unit} (ctx : both impl_574521470_) (state : both (t_OvnContractState v_G (both uint_size))) : both (t_Result (v_A × t_OvnContractState v_G (both uint_size)) t_ParseError) :=
-  cast_vote ctx state  :=
+Equations impl__cast_vote {v_G : _} {n : both uint_size} {v_A : _} {impl_574521470_ : _} `{ t_Sized v_G} `{ t_Group v_G} `{ t_Sized v_A} `{ t_Sized impl_574521470_} `{ t_HasActions v_A} `{ t_HasReceiveContext impl_574521470_ 'unit} (ctx : both impl_574521470_) (state : both (t_OvnContractState v_G (both uint_size))) : both (t_Result (v_A × t_OvnContractState v_G (both uint_size)) t_ParseError) :=
+  impl__cast_vote ctx state  :=
     run (letb '(_,out) := f_get (f_parameter_cursor ctx) in
     letm[choice_typeMonad.result_bind_code t_ParseError] (params : t_CastVoteParam f_Z) := out in
-    Result_Ok (letb g_pow_yi := compute_g_pow_yi (cast_int (WS2 := _) (f_cvp_i params)) (f_g_pow_xis state) in
-    letb g_pow_xi_yi_vi := compute_group_element_for_vote (f_cvp_xi params) (f_cvp_vote params) g_pow_yi in
-    letb zkp_vi := zkp_one_out_of_two (f_cvp_zkp_random_w params) (f_cvp_zkp_random_r params) (f_cvp_zkp_random_d params) g_pow_yi (f_cvp_xi params) (f_cvp_vote params) in
+    Result_Ok (letb g_pow_yi := impl__compute_g_pow_yi (cast_int (WS2 := _) (f_cvp_i params)) (f_g_pow_xis state) in
+    letb g_pow_xi_yi_vi := impl__compute_group_element_for_vote (f_cvp_xi params) (f_cvp_vote params) g_pow_yi in
+    letb zkp_vi := impl__zkp_one_out_of_two (f_cvp_zkp_random_w params) (f_cvp_zkp_random_r params) (f_cvp_zkp_random_d params) g_pow_yi (f_cvp_xi params) (f_cvp_vote params) in
     letb cast_vote_state_ret := f_clone state in
     letb cast_vote_state_ret := Build_t_OvnContractState[cast_vote_state_ret] (f_g_pow_xi_yi_vis := update_at_usize (f_g_pow_xi_yi_vis cast_vote_state_ret) (cast_int (WS2 := _) (f_cvp_i params)) g_pow_xi_yi_vi) in
     letb cast_vote_state_ret := Build_t_OvnContractState[cast_vote_state_ret] (f_zkp_vis := update_at_usize (f_zkp_vis cast_vote_state_ret) (cast_int (WS2 := _) (f_cvp_i params)) zkp_vi) in
     Result_Ok (prod_b (f_accept,cast_vote_state_ret)))) : both (t_Result (v_A × t_OvnContractState v_G (both uint_size)) t_ParseError).
 Fail Next Obligation.
 
-Equations commit_to_vote {v_G : _} {n : both uint_size} {v_A : _} {impl_574521470_ : _} `{ t_Sized v_G} `{ t_Sized v_A} `{ t_Sized impl_574521470_} `{ t_Group v_G} `{ t_HasActions v_A} `{ t_HasReceiveContext impl_574521470_ 'unit} (ctx : both impl_574521470_) (state : both (t_OvnContractState v_G (both uint_size))) : both (t_Result (v_A × t_OvnContractState v_G (both uint_size)) t_ParseError) :=
-  commit_to_vote ctx state  :=
+Equations impl__commit_to_vote {v_G : _} {n : both uint_size} {v_A : _} {impl_574521470_ : _} `{ t_Sized v_G} `{ t_Group v_G} `{ t_Sized v_A} `{ t_Sized impl_574521470_} `{ t_HasActions v_A} `{ t_HasReceiveContext impl_574521470_ 'unit} (ctx : both impl_574521470_) (state : both (t_OvnContractState v_G (both uint_size))) : both (t_Result (v_A × t_OvnContractState v_G (both uint_size)) t_ParseError) :=
+  impl__commit_to_vote ctx state  :=
     run (letb '(_,out) := f_get (f_parameter_cursor ctx) in
     letm[choice_typeMonad.result_bind_code t_ParseError] (params : t_CastVoteParam f_Z) := out in
     Result_Ok (letb _ := foldi_both_list (f_into_iter (Build_t_Range (f_start := ret_both (0 : uint_size)) (f_end := n))) (fun i =>
       ssp (fun _ =>
-        ifb orb (not (schnorr_zkp_validate ((f_g_pow_xis state).a[i]) ((f_zkp_xis state).a[i]))) (not ((f_round1 state).a[i]))
-        then letm[choice_typeMonad.result_bind_code (t_Result (v_A × t_OvnContractState v_G (both uint_size)) t_ParseError)] hoist26 := ControlFlow_Break (Result_Err ParseError) in
-        ControlFlow_Continue (never_to_any hoist26)
+        ifb orb (not (impl__schnorr_zkp_validate ((f_g_pow_xis state).a[i]) ((f_zkp_xis state).a[i]))) (not ((f_round1 state).a[i]))
+        then letm[choice_typeMonad.result_bind_code (t_Result (v_A × t_OvnContractState v_G (both uint_size)) t_ParseError)] hoist30 := ControlFlow_Break (Result_Err ParseError) in
+        ControlFlow_Continue (never_to_any hoist30)
         else ControlFlow_Continue (ret_both (tt : 'unit)) : (both (t_ControlFlow (t_Result (v_A × t_OvnContractState v_G (both uint_size)) t_ParseError) 'unit)))) (ret_both (tt : 'unit)) in
-    letb g_pow_yi := compute_g_pow_yi (cast_int (WS2 := _) (f_cvp_i params)) (f_g_pow_xis state) in
-    letb g_pow_xi_yi_vi := compute_group_element_for_vote (f_cvp_xi params) (f_cvp_vote params) g_pow_yi in
-    letb commit_vi := commit_to g_pow_xi_yi_vi in
+    letb g_pow_yi := impl__compute_g_pow_yi (cast_int (WS2 := _) (f_cvp_i params)) (f_g_pow_xis state) in
+    letb g_pow_xi_yi_vi := impl__compute_group_element_for_vote (f_cvp_xi params) (f_cvp_vote params) g_pow_yi in
+    letb commit_vi := impl__commit_to g_pow_xi_yi_vi in
     letb commit_to_vote_state_ret := f_clone state in
     letb commit_to_vote_state_ret := Build_t_OvnContractState[commit_to_vote_state_ret] (f_commit_vis := update_at_usize (f_commit_vis commit_to_vote_state_ret) (cast_int (WS2 := _) (f_cvp_i params)) commit_vi) in
     Result_Ok (prod_b (f_accept,commit_to_vote_state_ret)))) : both (t_Result (v_A × t_OvnContractState v_G (both uint_size)) t_ParseError).
 Fail Next Obligation.
 
-Equations init_ovn_contract {v_G : _} {n : both uint_size} `{ t_Sized v_G} `{ t_Group v_G} (_ : both 'unit) : both (t_Result (t_OvnContractState v_G (both uint_size)) t_Reject) :=
-  init_ovn_contract _  :=
+Equations impl__init_ovn_contract {v_G : _} {n : both uint_size} `{ t_Sized v_G} `{ t_Group v_G} (_ : both 'unit) : both (t_Result (t_OvnContractState v_G (both uint_size)) t_Reject) :=
+  impl__init_ovn_contract _  :=
     Result_Ok (Build_t_OvnContractState (f_g_pow_xis := repeat f_group_one n) (f_zkp_xis := repeat (Build_t_SchnorrZKPCommit (f_schnorr_zkp_u := f_group_one) (f_schnorr_zkp_z := f_field_zero) (f_schnorr_zkp_c := f_field_zero)) n) (f_commit_vis := repeat f_field_zero n) (f_g_pow_xi_yi_vis := repeat f_group_one n) (f_zkp_vis := repeat (Build_t_OrZKPCommit (f_or_zkp_x := f_group_one) (f_or_zkp_y := f_group_one) (f_or_zkp_a1 := f_group_one) (f_or_zkp_b1 := f_group_one) (f_or_zkp_a2 := f_group_one) (f_or_zkp_b2 := f_group_one) (f_or_zkp_c := f_field_zero) (f_or_zkp_d1 := f_field_zero) (f_or_zkp_d2 := f_field_zero) (f_or_zkp_r1 := f_field_zero) (f_or_zkp_r2 := f_field_zero)) n) (f_tally := ret_both (0 : int32)) (f_round1 := repeat (ret_both (false : 'bool)) n)) : both (t_Result (t_OvnContractState v_G (both uint_size)) t_Reject).
 Fail Next Obligation.
 
-Equations register_vote {v_G : _} {n : both uint_size} {v_A : _} {impl_574521470_ : _} `{ t_Sized v_G} `{ t_Sized v_A} `{ t_Sized impl_574521470_} `{ t_Group v_G} `{ t_HasActions v_A} `{ t_HasReceiveContext impl_574521470_ 'unit} (ctx : both impl_574521470_) (state : both (t_OvnContractState v_G (both uint_size))) : both (t_Result (v_A × t_OvnContractState v_G (both uint_size)) t_ParseError) :=
-  register_vote ctx state  :=
+Equations impl__register_vote {v_G : _} {n : both uint_size} {v_A : _} {impl_574521470_ : _} `{ t_Sized v_G} `{ t_Group v_G} `{ t_Sized v_A} `{ t_Sized impl_574521470_} `{ t_HasActions v_A} `{ t_HasReceiveContext impl_574521470_ 'unit} (ctx : both impl_574521470_) (state : both (t_OvnContractState v_G (both uint_size))) : both (t_Result (v_A × t_OvnContractState v_G (both uint_size)) t_ParseError) :=
+  impl__register_vote ctx state  :=
     run (letb '(_,out) := f_get (f_parameter_cursor ctx) in
     letm[choice_typeMonad.result_bind_code t_ParseError] (params : t_RegisterParam f_Z) := out in
     Result_Ok (letb g_pow_xi := f_g_pow (f_rp_xi params) in
-    letb zkp_xi := schnorr_zkp (f_rp_zkp_random params) g_pow_xi (f_rp_xi params) in
+    letb zkp_xi := impl__schnorr_zkp (f_rp_zkp_random params) g_pow_xi (f_rp_xi params) in
     letb register_vote_state_ret := f_clone state in
     letb register_vote_state_ret := Build_t_OvnContractState[register_vote_state_ret] (f_g_pow_xis := update_at_usize (f_g_pow_xis register_vote_state_ret) (cast_int (WS2 := _) (f_rp_i params)) g_pow_xi) in
     letb register_vote_state_ret := Build_t_OvnContractState[register_vote_state_ret] (f_zkp_xis := update_at_usize (f_zkp_xis register_vote_state_ret) (cast_int (WS2 := _) (f_rp_i params)) zkp_xi) in
@@ -434,18 +451,18 @@ Equations register_vote {v_G : _} {n : both uint_size} {v_A : _} {impl_574521470
     Result_Ok (prod_b (f_accept,register_vote_state_ret)))) : both (t_Result (v_A × t_OvnContractState v_G (both uint_size)) t_ParseError).
 Fail Next Obligation.
 
-Equations tally_votes {v_G : _} {n : both uint_size} {v_A : _} {impl_574521470_ : _} `{ t_Sized v_G} `{ t_Sized v_A} `{ t_Sized impl_574521470_} `{ t_Group v_G} `{ t_HasActions v_A} `{ t_HasReceiveContext impl_574521470_ 'unit} (_ : both impl_574521470_) (state : both (t_OvnContractState v_G (both uint_size))) : both (t_Result (v_A × t_OvnContractState v_G (both uint_size)) t_ParseError) :=
-  tally_votes _ state  :=
+Equations impl__tally_votes {v_G : _} {n : both uint_size} {v_A : _} {impl_574521470_ : _} `{ t_Sized v_G} `{ t_Group v_G} `{ t_Sized v_A} `{ t_Sized impl_574521470_} `{ t_HasActions v_A} `{ t_HasReceiveContext impl_574521470_ 'unit} (_ : both impl_574521470_) (state : both (t_OvnContractState v_G (both uint_size))) : both (t_Result (v_A × t_OvnContractState v_G (both uint_size)) t_ParseError) :=
+  impl__tally_votes _ state  :=
     letb _ := foldi_both_list (f_into_iter (Build_t_Range (f_start := ret_both (0 : uint_size)) (f_end := n))) (fun i =>
       ssp (fun _ =>
-        letb g_pow_yi := compute_g_pow_yi i (f_g_pow_xis state) in
-        letm[choice_typeMonad.result_bind_code (t_Result (v_A × t_OvnContractState v_G (both uint_size)) t_ParseError)] _ := ControlFlow_Continue (ifb not (zkp_one_out_of_two_validate g_pow_yi ((f_zkp_vis state).a[i]))
-        then letm[choice_typeMonad.result_bind_code (t_Result (v_A × t_OvnContractState v_G (both uint_size)) t_ParseError)] hoist27 := ControlFlow_Break (Result_Err ParseError) in
-        ControlFlow_Continue (never_to_any hoist27)
+        letb g_pow_yi := impl__compute_g_pow_yi i (f_g_pow_xis state) in
+        letm[choice_typeMonad.result_bind_code (t_Result (v_A × t_OvnContractState v_G (both uint_size)) t_ParseError)] _ := ControlFlow_Continue (ifb not (impl__zkp_one_out_of_two_validate g_pow_yi ((f_zkp_vis state).a[i]))
+        then letm[choice_typeMonad.result_bind_code (t_Result (v_A × t_OvnContractState v_G (both uint_size)) t_ParseError)] hoist31 := ControlFlow_Break (Result_Err ParseError) in
+        ControlFlow_Continue (never_to_any hoist31)
         else ControlFlow_Continue (ret_both (tt : 'unit))) in
-        ifb not (check_commitment ((f_g_pow_xi_yi_vis state).a[i]) ((f_commit_vis state).a[i]))
-        then letm[choice_typeMonad.result_bind_code (t_Result (v_A × t_OvnContractState v_G (both uint_size)) t_ParseError)] hoist28 := ControlFlow_Break (Result_Err ParseError) in
-        ControlFlow_Continue (never_to_any hoist28)
+        ifb not (impl__check_commitment ((f_g_pow_xi_yi_vis state).a[i]) ((f_commit_vis state).a[i]))
+        then letm[choice_typeMonad.result_bind_code (t_Result (v_A × t_OvnContractState v_G (both uint_size)) t_ParseError)] hoist32 := ControlFlow_Break (Result_Err ParseError) in
+        ControlFlow_Continue (never_to_any hoist32)
         else ControlFlow_Continue (ret_both (tt : 'unit)) : (both (t_ControlFlow (t_Result (v_A × t_OvnContractState v_G (both uint_size)) t_ParseError) 'unit)))) (ret_both (tt : 'unit)) in
     letb vote_result := f_group_one in
     letb vote_result := foldi_both_list (f_into_iter (f_g_pow_xi_yi_vis state)) (fun g_pow_vote =>
